Reformulate pborrow using cif

nola/iris/pborrow.v
@@ -2,160 +2,83 @@
 
 From nola.bi Require Export plist.
 From nola.bi Require Import order.
-From nola.iris Require Export borrow proph_ag.
+From nola.iris Require Export borrow proph_ag cif.
 From iris.proofmode Require Import proofmode.
-Import ProdNotation PlistNotation FunPNotation iPropAppNotation LftNotation
-  ProphNotation ModwNotation.
+Import ProdNotation PlistNotation FunPNotation BUpd0Notation iPropAppNotation
+  LftNotation ProphNotation ModwNotation DsemNotation.
 
 Implicit Type (TY : synty) (FML : oFunctor) (α : lft) (q : Qp).
 
-(** Formula for prophetic borrowing *)
-Local Definition pborrow_fml TY FML : oFunctor :=
-  (* Just a formula *) FML +
-  (* For prophetic borrower *)
-  { X : TY & leibnizO (gname *' prvar X) * (X -d> FML) } +
-  (* For prophetic lender *)
-  { X : TY & leibnizO (clair TY X) * (X -d> FML) } +
-  (* For prophetic reborrowing *)
-  leibnizO (gname *' gname *' gname *'
-    { X : TY & prvar X *' { Y : TY & Y → X }}).
-Local Notation xjust Px := (inl (inl (inl Px))).
-Local Notation xjustf := (λ Px, xjust Px).
-Local Notation xpbor X γ ξ Φx := (inl (inl (inr (existT X ((γ, ξ)', Φx))))).
-Local Notation xplend X xπ Φx := (inl (inr (existT X (xπ, Φx)))).
-Local Notation xpreborrow X Y γ γ' γx ξ f :=
-  (inr (γ, γ', γx, existT X (ξ, existT Y f)')').
-
-(** Ghost state *)
-Class pborrowGS TY FML Σ := PborrowGS {
-  pborrowGS_borrow :: borrowGS (pborrow_fml TY FML) Σ;
-  pborrowGS_proph :: prophGS TY Σ;
-  pborrowGS_proph_ag : proph_agG TY Σ;
-}.
-Local Existing Instance pborrowGS_proph_ag.
-Class pborrowGpreS TY FML Σ := PborrowGpreS {
-  pborrowGpreS_borrow :: borrowGpreS (pborrow_fml TY FML) Σ;
-  pborrowGpreS_proph :: prophGpreS TY Σ;
-  pborrowGpreS_proph_ag : proph_agG TY Σ;
-}.
-Local Existing Instance pborrowGpreS_proph_ag.
-Definition pborrowΣ TY FML `{!oFunctorContractive FML} :=
-  #[borrowΣ (pborrow_fml TY FML); prophΣ TY; proph_agΣ TY].
-#[export] Instance subG_pborrow
-  `{!oFunctorContractive FML, !subG (pborrowΣ TY FML) Σ} :
-  pborrowGpreS TY FML Σ.
-Proof. solve_inG. Qed.
-
 Section pborrow.
-  Context `{!pborrowGS TY FML Σ, !@ModUpd (iProp Σ) M, !ModBUpd M}.
-  Implicit Type (sm : FML $oi Σ -d> iProp Σ) (X Y : TY) (Xl Yl : list TY)
-    (Px : FML $oi Σ) (Pb : pborrow_fml TY FML $oi Σ).
+  Context `{!borrowGS (cifOF CON) Σ, !prophGS TY Σ, !proph_agG TY Σ}.
+  Implicit Type (γ : positive) (X Y : TY) (Xl Yl : list TY) (Px : cif CON Σ).
 
   (** ** Tokens *)
 
-  (** Non-prophetic tokens *)
-  Definition nbor_tok α Px : iProp Σ := bor_tok α (xjust Px).
-  Definition nobor_tok α q Px : iProp Σ := obor_tok α q (xjust Px).
-  Definition nlend_tok α Px : iProp Σ := lend_tok α (xjust Px).
+  (** Formulas for a borrower and a lender *)
+  Local Definition cif_xpbor {X} γ ξ (Φx : X -d> cif CON Σ) : cif CON Σ :=
+    ∃ x, ▷ proph_ctrl γ x ξ ∗ Φx x.
+  Local Definition cif_xplend {X} (xπ : clair TY X) (Φx : X -d> cif CON Σ)
+    : cif CON Σ :=
+    ∃ x, ▷ ⟨π, xπ π = x⟩ ∗ Φx x.
+
+  (** Formulas are non-expansive *)
+  Local Instance cif_pbor_ne {X γ ξ} : NonExpansive (@cif_xpbor X γ ξ).
+  Proof. unfold cif_xpbor. solve_proper. Qed.
+  Local Instance cif_plend_ne {X xπ} : NonExpansive (@cif_xplend X xπ).
+  Proof. unfold cif_xplend. solve_proper. Qed.
 
   (** Prophetic borrower token *)
   Local Definition pbor_tok_def {X} α (x : X) (ξ : prvar X)
-    (Φx : X -d> FML $oi Σ) : iProp Σ :=
-    [†α] ∨ ∃ γ, val_obs γ x ∗ bor_tok α (xpbor X γ ξ Φx).
+    (Φx : X -d> cif CON Σ) : iProp Σ :=
+    [†α] ∨ ∃ γ, val_obs γ x ∗ bor_tok α (cif_xpbor γ ξ Φx).
   Local Lemma pbor_tok_aux : seal (@pbor_tok_def). Proof. by eexists. Qed.
   Definition pbor_tok {X} := pbor_tok_aux.(unseal) X.
   Local Lemma pbor_tok_unseal : @pbor_tok = @pbor_tok_def.
   Proof. exact: seal_eq. Qed.
 
   (** Open prophetic borrower token *)
-  Local Definition pobor_tok_def {X} α q (ξ : prvar X) (Φx : X -d> FML $oi Σ)
+  Local Definition pobor_tok_def {X} α q (ξ : prvar X) (Φx : X -d> cif CON Σ)
     : iProp Σ :=
     ∃ γ, (∃ x, val_obs γ x ∗ proph_ctrl γ x ξ) ∗
-      obor_tok α q (xpbor X γ ξ Φx).
+      obor_tok α q (cif_xpbor γ ξ Φx).
   Local Lemma pobor_tok_aux : seal (@pobor_tok_def). Proof. by eexists. Qed.
   Definition pobor_tok {X} := pobor_tok_aux.(unseal) X.
   Local Lemma pobor_tok_unseal : @pobor_tok = @pobor_tok_def.
   Proof. exact: seal_eq. Qed.
 
   (** Prophetic lender token *)
-  Definition plend_tok {X} α (xπ : clair TY X) (Φx : X -d> FML $oi Σ)
-    : iProp Σ := lend_tok α (xplend X xπ Φx).
+  Definition plend_tok {X} α (xπ : clair TY X) (Φx : X -d> cif CON Σ)
+    : iProp Σ :=
+    lend_tok α (cif_xplend xπ Φx).
 
   (** Borrower and lender tokens are non-expansive *)
-  #[export] Instance nbor_tok_ne {α} : NonExpansive (nbor_tok α).
-  Proof. solve_proper. Qed.
-  #[export] Instance nbor_tok_proper {α} : Proper ((≡) ==> (⊣⊢)) (nbor_tok α).
-  Proof. apply ne_proper, _. Qed.
-  #[export] Instance nobor_tok_ne {α q} : NonExpansive (nobor_tok α q).
-  Proof. solve_proper. Qed.
-  #[export] Instance nobor_tok_proper {α q} :
-    Proper ((≡) ==> (⊣⊢)) (nobor_tok α q).
-  Proof. apply ne_proper, _. Qed.
-  #[export] Instance nlend_tok_ne {α} : NonExpansive (nlend_tok α).
-  Proof. solve_proper. Qed.
-  #[export] Instance nlend_tok_proper {α} : Proper ((≡) ==> (⊣⊢)) (nlend_tok α).
-  Proof. apply ne_proper, _. Qed.
   #[export] Instance pbor_tok_ne {X α x ξ} :
     NonExpansive (pbor_tok (X:=X) α x ξ).
-  Proof.
-    rewrite pbor_tok_unseal /pbor_tok_def=> ????. do 7 f_equiv.
-    apply inr_ne. by apply: existT_ne.
-  Qed.
+  Proof. rewrite pbor_tok_unseal. solve_proper. Qed.
   #[export] Instance pbor_tok_proper {X α x ξ} :
     Proper ((≡) ==> (⊣⊢)) (pbor_tok (X:=X) α x ξ).
   Proof. apply ne_proper, _. Qed.
   #[export] Instance pobor_tok_ne {X α q ξ} :
     NonExpansive (pobor_tok (X:=X) α q ξ).
-  Proof.
-    rewrite pobor_tok_unseal /pobor_tok_def=> ????. do 6 f_equiv.
-    apply inr_ne. by apply: existT_ne.
-  Qed.
+  Proof. rewrite pobor_tok_unseal. solve_proper. Qed.
   #[export] Instance pobor_tok_proper {X α q ξ} :
     Proper ((≡) ==> (⊣⊢)) (pobor_tok (X:=X) α q ξ).
   Proof. apply ne_proper, _. Qed.
   #[export] Instance plend_tok_ne {X α xπ} :
     NonExpansive (plend_tok (X:=X) α xπ).
-  Proof.
-    unfold plend_tok=> ????. do 2 f_equiv. apply inr_ne. by apply: existT_ne.
-  Qed.
+  Proof. solve_proper. Qed.
   #[export] Instance plend_tok_proper {X α xπ} :
     Proper ((≡) ==> (⊣⊢)) (plend_tok (X:=X) α xπ).
   Proof. apply ne_proper, _. Qed.
 
-  (** Borrower and lender tokens are timeless for discrete formulas *)
-  #[export] Instance nbor_tok_timeless `{!Discrete Px} {α} :
-    Timeless (nbor_tok α Px).
-  Proof. exact _. Qed.
-  #[export] Instance nobor_tok_timeless `{!Discrete Px} {α q} :
-    Timeless (nobor_tok α q Px).
-  Proof. exact _. Qed.
-  #[export] Instance nlend_tok_timeless `{!Discrete Px} {α} :
-    Timeless (nlend_tok α Px).
-  Proof. exact _. Qed.
-  #[export] Instance pbor_tok_timeless `{!Discrete (Φx : X -d> _)} {α x ξ} :
-    Timeless (pbor_tok α x ξ Φx).
-  Proof. rewrite pbor_tok_unseal. exact _. Qed.
-  #[export] Instance pobor_tok_timeless `{!Discrete (Φx : X -d> _)} {α q ξ} :
-    Timeless (pobor_tok α q ξ Φx).
-  Proof. rewrite pobor_tok_unseal. exact _. Qed.
-  #[export] Instance plend_tok_timeless `{!Discrete (Φx : X -d> _)} {α xπ} :
-    Timeless (plend_tok α xπ Φx).
-  Proof. exact _. Qed.
+  (** ** Basic lemmas *)
 
   (** Fake a borrower token from the dead lifetime token *)
-  Lemma nbor_tok_fake {α} Px : [†α] ⊢ nbor_tok α Px.
-  Proof. exact: bor_tok_fake. Qed.
   Lemma pbor_tok_fake {X α} x ξ Φx : [†α] ⊢ pbor_tok (X:=X) α x ξ Φx.
   Proof. rewrite pbor_tok_unseal. iIntros. by iLeft. Qed.
 
   (** Modify the lifetime of borrower and lender tokens *)
-  Lemma nbor_tok_lft {α β Px} : β ⊑□ α -∗ nbor_tok α Px -∗ nbor_tok β Px.
-  Proof. exact bor_tok_lft. Qed.
-  Lemma nobor_tok_lft {α β q r Px} :
-    β ⊑□ α -∗ (q.[α] -∗ r.[β]) -∗ nobor_tok α q Px -∗ nobor_tok β r Px.
-  Proof. exact obor_tok_lft. Qed.
-  Lemma nlend_tok_lft {α β Px} : α ⊑□ β -∗ nlend_tok α Px -∗ nlend_tok β Px.
-  Proof. exact lend_tok_lft. Qed.
   Lemma pbor_tok_lft {X α β x ξ Φx} :
     β ⊑□ α -∗ pbor_tok (X:=X) α x ξ Φx -∗ pbor_tok β x ξ Φx.
   Proof.
@@ -184,167 +107,24 @@ Section pborrow.
     iApply (vo_proph_pc with "vo' ξ").
   Qed.
 
-  (** ** World satisfaction *)
+  (** ** Borrows *)
 
-  (** Body of a prophetic lender *)
-  Definition plend_body sm {X} (xπ : clair TY X) (Φx : X -d> FML $oi Σ)
-    : iProp Σ := ∃ x', ⟨π, xπ π = x'⟩ ∗ sm (Φx x').
-  Definition plend_body_var sm {X} (ξ : prvar X) (Φx : X -d> FML $oi Σ)
-    : iProp Σ := plend_body sm (λ π, π ξ) Φx.
-  (** [plend_body] is non-expansive *)
-  #[export] Instance plend_body_ne `{!NonExpansive sm} {X n} :
-    Proper ((=) ==> (≡{n}≡) ==> (≡{n}≡)) (@plend_body sm X).
-  Proof. solve_proper. Qed.
-
-  (** Semantics of [pborrow_fml] *)
-  Local Definition pbsem sm : _ -d> iProp Σ := λ Pb, match Pb with
-    | xjust Px => sm Px
-    | xpbor _ γ ξ Φx => ∃ x, proph_ctrl γ x ξ ∗ sm (Φx x)
-    | xplend _ xπ Φx => plend_body sm xπ Φx
-    | xpreborrow _ _ γ γ' γx ξ f =>
-        ∃ y, proph_ctrl γ (f y) ξ ∗ val_obs γ' y ∗ val_obs γx y
-    end%I.
-
-  (** [pbsem] is non-expansive *)
-  Local Instance pbsem_ne : NonExpansive pbsem.
-  Proof. move=> ????[[[?|[?[??]]]|[?[??]]]|?]//=; solve_proper. Qed.
-  (** [pbsem sm] is non-expansive if [sm] is *)
-  Local Lemma pbsem_sem_ne {sm} :
-    internal_ne sm ⊢@{iProp Σ} internal_ne (pbsem sm).
-  Proof.
-    iIntros "#Ne" ([s|?][s'|?]) "≡"; rewrite sum_equivI //=; [|by iRewrite "≡"].
-    rewrite sum_equivI; case: s=> [s|[?[? Φx]]]; case: s'=> [s'|[?[??]]]//=;
-      last first.
-    { rewrite sigT_equivI /=. iDestruct "≡" as (?) "≡". subst=>/=.
-      rewrite prod_equivI /= discrete_fun_equivI.
-      iDestruct "≡" as "[<- ≡]". iApply f_equivI_exist. iIntros (x).
-      by iRewrite ("Ne" $! (Φx x) with "≡"). }
-    rewrite sum_equivI; case: s=> [?|[?[? Φx]]]; case: s'=> [?|[?[??]]]//=.
-    { iApply ("Ne" with "≡"). }
-    rewrite sigT_equivI /=. iDestruct "≡" as (?) "≡". subst=>/=.
-    rewrite prod_equivI /= discrete_fun_equivI. iDestruct "≡" as "[<- ≡]".
-    iApply f_equivI_exist. iIntros (x). by iRewrite ("Ne" $! (Φx x) with "≡").
-  Qed.
-
-  (** World satisfaction *)
-  Definition pborrow_wsat M sm : iProp Σ := borrow_wsat M (pbsem sm).
-
-  (** [pborrow_wsat] is non-expansive *)
-  #[export] Instance pborrow_wsat_ne {n} :
-    Proper (((≡{n}≡) ==> (≡{n}≡)) ==> (≡{n}≡) ==> (≡{n}≡)) pborrow_wsat.
-  Proof. solve_proper. Qed.
-  (** [pborrow_wsat] is monotone over the modality *)
-  #[export] Instance pborrow_wsat_mono :
-    Mono (OT:=_-p>_ : bi) (OT':=_-p>_ : bi) pborrow_wsat.
-  Proof. move=> ????. by apply: borrow_wsat_mono. Qed.
-
-  (** ** For non-prophetic borrowing *)
-
-  (** Create new borrowers and lenders *)
-  Lemma nbor_nlend_tok_new_list {sm} α Pxl Qxl :
-    ([∗ list] Px ∈ Pxl, sm Px) -∗
-    ([†α] -∗ ([∗ list] Px ∈ Pxl, sm Px) -∗ M
-      ([∗ list] Qx ∈ Qxl, sm Qx)%I) =[pborrow_wsat M sm]=∗
-      ([∗ list] Px ∈ Pxl, nbor_tok α Px) ∗ [∗ list] Qx ∈ Qxl, nlend_tok α Qx.
-  Proof.
-    iIntros "Pxl →Qxl".
-    iMod (bor_lend_tok_new_list (M:=M) (sm:=pbsem _) α
-      (xjustf <$> Pxl) (xjustf <$> Qxl) with "[Pxl] [→Qxl]");
-      by rewrite !big_sepL_fmap.
-  Qed.
-  Lemma nbor_nlend_tok_new {sm} α Px :
-    sm Px =[pborrow_wsat M sm]=∗ nbor_tok α Px ∗ nlend_tok α Px.
-  Proof.
-    iIntros "Px". iMod (nbor_nlend_tok_new_list α [Px] [Px] with "[Px] []")
-      as "[[$_][$_]]"; by [iFrame|iIntros|].
-  Qed.
-
-  (** Split a lender *)
-  Lemma nlend_tok_split {sm α Px} Qxl :
-    nlend_tok α Px -∗ (sm Px -∗ M ([∗ list] Qx ∈ Qxl, sm Qx))
-      =[pborrow_wsat M sm]=∗ [∗ list] Qx ∈ Qxl, nlend_tok α Qx.
-  Proof.
-    iIntros "l →Qxl".
-    iMod (lend_tok_split (M:=M) (sm:=pbsem _) (xjustf <$> Qxl)
-      with "l [→Qxl]"); by rewrite !big_sepL_fmap.
-  Qed.
-
-  (** Retrieve from a lender *)
-  Lemma nlend_tok_retrieve {sm α Px} :
-    [†α] -∗ nlend_tok α Px -∗ modw M (pborrow_wsat M sm) (sm Px).
-  Proof. exact lend_tok_retrieve. Qed.
-
-  (** Open a borrower *)
-  Lemma nbor_tok_open {sm α q Px} :
-    q.[α] -∗ nbor_tok α Px -∗ modw M (pborrow_wsat M sm)
-      (nobor_tok α q Px ∗ sm Px).
-  Proof. exact bor_tok_open. Qed.
-
-  (** Merge and subdivide/reborrow borrowers *)
-  Lemma nobor_tok_merge_subdiv {sm} αqPxl Qxl β :
-    ([∗ list] '(α, q, Px)' ∈ αqPxl, β ⊑□ α ∗ nobor_tok α q Px) -∗
-    ([∗ list] Qx ∈ Qxl, sm Qx) -∗ ([†β] -∗ ([∗ list] Qx ∈ Qxl, sm Qx) -∗ M
-      ([∗ list] '(_, _, Px)' ∈ αqPxl, sm Px)%I) =[pborrow_wsat M sm]=∗
-      ([∗ list] '(α, q, Px)' ∈ αqPxl, q.[α] ∗ ([†β] -∗ nbor_tok α Px)) ∗
-      [∗ list] Qx ∈ Qxl, nbor_tok β Qx.
-  Proof.
-    iIntros "ol Qxl →Pxl".
-    iMod (obor_tok_merge_subdiv (M:=M) (sm:=pbsem _)
-      ((λ '(α, q, Px)', (α, q, xjust Px)') <$> αqPxl) (xjustf <$> Qxl)
-      with "[ol] [Qxl] [→Pxl]"); by rewrite !big_sepL_fmap /=.
-  Qed.
-  (** Subdivide/reborrow a borrower *)
-  Lemma nobor_tok_subdiv {sm α q Px} Qxl β :
-    β ⊑□ α -∗ nobor_tok α q Px -∗ ([∗ list] Qx ∈ Qxl, sm Qx) -∗
-    ([†β] -∗ ([∗ list] Qx ∈ Qxl, sm Qx) -∗ M (sm Px))
-      =[pborrow_wsat M sm]=∗
-      q.[α] ∗ ([†β] -∗ nbor_tok α Px) ∗ [∗ list] Qx ∈ Qxl, nbor_tok β Qx.
-  Proof.
-    iIntros "⊑ o Qxl →Px".
-    iMod (nobor_tok_merge_subdiv [(_,_,_)'] with "[⊑ o] Qxl [→Px]")
-      as "[[[$$]_]$]"=>/=; by [iFrame|rewrite bi.sep_emp|].
-  Qed.
-
-  (** Reborrow a borrower *)
-  Lemma nobor_tok_reborrow {sm α q Px} β :
-    β ⊑□ α -∗ nobor_tok α q Px -∗ sm Px =[pborrow_wsat M sm]=∗
-      q.[α] ∗ ([†β] -∗ nbor_tok α Px) ∗ nbor_tok β Px.
-  Proof.
-    iIntros "⊑ o Px".
-    iMod (nobor_tok_subdiv [Px] with "⊑ o [Px] []") as "($ & $ & $ & _)"=>/=;
-      by [iFrame|iIntros "_ [$ _]"|].
-  Qed.
-  Lemma nbor_tok_reborrow {sm α q Px} β :
-    β ⊑□ α -∗ q.[α] -∗ nbor_tok α Px -∗ modw M (pborrow_wsat M sm)
-      (q.[α] ∗ ([†β] -∗ nbor_tok α Px) ∗ nbor_tok β Px).
-  Proof.
-    iIntros "⊑ α b". iMod (nbor_tok_open with "α b") as "[o Px]".
-    by iMod (nobor_tok_reborrow with "⊑ o Px").
-  Qed.
-  (** Simply close a borrower *)
-  Lemma nobor_tok_close {sm α q Px} :
-    nobor_tok α q Px -∗ sm Px =[pborrow_wsat M sm]=∗ q.[α] ∗ nbor_tok α Px.
-  Proof.
-    iIntros "o Px".
-    iMod (nobor_tok_reborrow with "[] o Px") as "($ & _ & $)";
-      by [iApply lft_sincl_refl|].
-  Qed.
-
-  (** ** On prophetic borrowing *)
+  Context `{!SemCifcon JUDG CON Σ, !@ModUpd (iProp Σ) M, !ModBUpd M,
+    !ModExcept0 M}.
+  Implicit Type δ : JUDG -n> iProp Σ.
 
   (** Utility *)
-  Local Definition pbor_list {Xl}
-    (γξxΦxl : plist (λ X, _ *' _ *' X *' (X → _)) Xl)
-    : list (pborrow_fml TY FML $oi Σ) :=
-    of_plist (λ _ '(γ, ξ, _, Φx)', xpbor _ γ ξ Φx) γξxΦxl.
-  Local Definition plend_list {Xl} (xπΦxl : plist (λ X, _ *' (X → _)) Xl)
-    : list (pborrow_fml TY FML $oi Σ) :=
-    of_plist (λ _ '(xπ, Φx)', xplend _ xπ Φx) xπΦxl.
-  Local Lemma vo_pbor_alloc_list {sm Xl ξl} {xΦxl : plist _ Xl} :
-    1:∗[of_plist_prvar ξl] -∗ ([∗ plist] '(x, Φx)' ∈ xΦxl, sm (Φx x)) ==∗ ∃ γl,
-      let γξxΦxl := plist_zip γl (plist_zip ξl xΦxl) in
+  Local Definition cif_xpbors {Xl}
+    (γξxΦxl : plist (λ X, _ *' _ *' X *' (X → _)) Xl) : list (cif CON Σ) :=
+    of_plist (λ _ '(γ, ξ, _, Φx)', cif_xpbor γ ξ Φx) γξxΦxl.
+  Local Definition cif_xplends {Xl} (xπΦxl : plist (λ X, _ *' (X → _)) Xl)
+    : list (cif CON Σ) :=
+    of_plist (λ _ '(xπ, Φx)', cif_xplend xπ Φx) xπΦxl.
+  Local Lemma vo_pbor_alloc_list {δ Xl ξl} {xΦxl : plist _ Xl} :
+    1:∗[of_plist_prvar ξl] -∗ ([∗ plist] '(x, Φx)' ∈ xΦxl, ⟦ Φx x ⟧(δ)) ==∗
+      ∃ γl, let γξxΦxl := plist_zip γl (plist_zip ξl xΦxl) in
       ([∗ plist] '(γ, _, x, _)' ∈ γξxΦxl, val_obs γ x) ∗
-      ([∗ list] Pb ∈ pbor_list γξxΦxl, pbsem sm Pb).
+      ([∗ list] Px ∈ cif_xpbors γξxΦxl, ⟦ Px ⟧(δ)).
   Proof.
     elim: Xl ξl xΦxl=>/=; [iIntros; by iExists ()|].
     move=> X Xl IH [ξ ξl] [[x Φx] xΦxl]. iIntros "[ξ ξl] [Φx Φxl]".
@@ -353,23 +133,40 @@ Section pborrow.
     iFrame "vo vol pborl". iExists _. iFrame.
   Qed.
 
+  (** Body of a lender *)
+  Definition xplend {X} δ (xπ : clair TY X) (Φx : X -d> cif CON Σ) : iProp Σ :=
+    ∃ x, ▷ ⟨π, xπ π = x⟩ ∗ ⟦ Φx x ⟧(δ).
+  Definition xplend_var {X} δ (ξ : prvar X) (Φx : X -d> cif CON Σ) : iProp Σ :=
+    xplend δ (λ π, π ξ) Φx.
+  (** [xplend] and [xplend_var] are non-expansive *)
+  #[export] Instance xplend_ne {X δ xπ} : NonExpansive (@xplend X δ xπ).
+  Proof. solve_proper. Qed.
+  #[export] Instance xplend_proper {X δ xπ} :
+    Proper ((≡) ==> (≡)) (@xplend X δ xπ).
+  Proof. solve_proper. Qed.
+  #[export] Instance xplend_var_ne {X δ ξ} : NonExpansive (@xplend_var X δ ξ).
+  Proof. solve_proper. Qed.
+  #[export] Instance xplend_var_proper {X δ ξ} :
+    Proper ((≡) ==> (≡)) (@xplend_var X δ ξ).
+  Proof. solve_proper. Qed.
+
   (** Lemma for [pbor_plend_tok_new_list] *)
-  Local Lemma pbor_list_sem_to_plend {sm Xl γl} {ξxΦxl : plist _ Xl} :
-    ([∗ list] Pb ∈ pbor_list (plist_zip γl ξxΦxl), pbsem sm Pb) ==∗
-      [∗ plist] '(ξ, _, Φx)' ∈ ξxΦxl, plend_body_var sm ξ Φx.
+  Local Lemma cif_xpbors_sem_to_plend {δ Xl γl} {ξxΦxl : plist _ Xl} :
+    ([∗ list] Px ∈ cif_xpbors (plist_zip γl ξxΦxl), ⟦ Px ⟧(δ)) ==∗◇
+      [∗ plist] '(ξ, _, Φx)' ∈ ξxΦxl, xplend_var δ ξ Φx.
   Proof.
     elim: Xl γl ξxΦxl=>/=; [by iIntros|]=> X Xl IH [γ γl] [[ξ[x Φx]] ξxΦxl].
-    iIntros "[[%[pc Φx]] pborl]". iMod (IH with "pborl") as "$".
-    iMod (pc_resolve with "pc") as "?". iModIntro. iExists _. iFrame.
+    iIntros "[[%[>pc Φx]] pborl]". iMod (IH with "pborl") as "$".
+    iMod (pc_resolve with "pc"). iModIntro. iExists _. iFrame.
   Qed.
   (** Create new prophetic borrowers and lenders *)
-  Lemma pbor_plend_tok_new_list {sm} Xl α (xΦxl : plist _ Xl) :
+  Lemma pbor_plend_tok_new_list {δ} Xl α (xΦxl : plist _ Xl) :
     ⊢ |==> ∃ ξl, ∀ Yl (yπΨxl : plist (λ Y, _ *' (Y → _)) Yl),
       let ξxΦxl := plist_zip ξl xΦxl in
-      ([∗ plist] '(x, Φx)' ∈ xΦxl, sm (Φx x)) -∗
-      ([†α] -∗ ([∗ plist] '(ξ, _, Φx)' ∈ ξxΦxl, plend_body_var sm ξ Φx) -∗
-        M ([∗ plist] '(yπ, Ψx)' ∈ yπΨxl, plend_body sm yπ Ψx))
-        =[pborrow_wsat M sm]=∗
+      ([∗ plist] '(x, Φx)' ∈ xΦxl, ⟦ Φx x ⟧(δ)) -∗
+      ([†α] -∗ ([∗ plist] '(ξ, _, Φx)' ∈ ξxΦxl, xplend_var δ ξ Φx) -∗
+        M ([∗ plist] '(yπ, Ψx)' ∈ yπΨxl, xplend δ yπ Ψx))
+        =[borrow_wsat M ⟦⟧(δ)]=∗◇
         ([∗ plist] '(ξ, x, Φx)' ∈ ξxΦxl, pbor_tok α x ξ Φx) ∗
         ([∗ plist] '(yπ, Ψx)' ∈ yπΨxl, plend_tok α yπ Ψx).
   Proof.
@@ -377,10 +174,10 @@ Section pborrow.
     iModIntro. iExists ξl. iIntros (??) "Φxl →Ψxl".
     set ξxΦxl := plist_zip ξl xΦxl.
     iMod (vo_pbor_alloc_list with "ξl Φxl") as (γl) "[vol pborl]".
-    iMod (bor_lend_tok_new_list (M:=M) α _ (plend_list yπΨxl)
+    iMod (bor_lend_tok_new_list (FML:=cifOF _) (M:=M) α _ (cif_xplends yπΨxl)
       with "pborl [→Ψxl]") as "[bl ll]".
     { iStopProof. f_equiv. iIntros "→Ψxl pborl".
-      iMod (pbor_list_sem_to_plend with "pborl"). rewrite big_sepL_of_plist.
+      iMod (cif_xpbors_sem_to_plend with "pborl"). rewrite big_sepL_of_plist.
       by iApply "→Ψxl". }
     iModIntro. rewrite !big_sepL_of_plist /=. iFrame "ll".
     iDestruct (big_sepPL_sep_2 with "vol bl") as "vobl".
@@ -389,8 +186,8 @@ Section pborrow.
     rewrite pbor_tok_unseal. iRight. iExists _. iFrame.
   Qed.
   (** Simply create a prophetic borrower and a prophetic lender *)
-  Lemma pbor_plend_tok_new {sm} X α x Φx :
-    sm (Φx x) =[pborrow_wsat M sm]=∗ ∃ ξ,
+  Lemma pbor_plend_tok_new {δ} X α x Φx :
+    ⟦ Φx x ⟧(δ) =[borrow_wsat M ⟦⟧(δ)]=∗◇ ∃ ξ,
       pbor_tok (X:=X) α x ξ Φx ∗ plend_tok α (λ π, π ξ) Φx.
   Proof.
     iIntros "Φx".
@@ -401,32 +198,31 @@ Section pborrow.
   Qed.
 
   (** Split a prophetic lender *)
-  Lemma plend_tok_split {sm X α xπ Φx} Yl
+  Lemma plend_tok_split {δ X α xπ Φx} Yl
     (yπΨxl : plist (λ Y, _ *' (Y → _)) Yl) :
     plend_tok (X:=X) α xπ Φx -∗
-    (plend_body sm xπ Φx -∗
-      M ([∗ plist] '(yπ, Ψx)' ∈ yπΨxl, plend_body sm yπ Ψx))
-      =[pborrow_wsat M sm]=∗ [∗ plist] '(yπ, Ψx)' ∈ yπΨxl, plend_tok α yπ Ψx.
+    (xplend δ xπ Φx -∗ M ([∗ plist] '(yπ, Ψx)' ∈ yπΨxl, xplend δ yπ Ψx))
+      =[borrow_wsat M ⟦⟧(δ)]=∗◇ [∗ plist] '(yπ, Ψx)' ∈ yπΨxl, plend_tok α yπ Ψx.
   Proof.
     iIntros "/=l →Ψxl".
-    iMod (lend_tok_split (M:=M) (sm:=pbsem _) (plend_list yπΨxl)
+    iMod (lend_tok_split (FML:=cifOF _) (M:=M) (cif_xplends yπΨxl)
       with "l [→Ψxl]"); by rewrite big_sepL_of_plist.
   Qed.
 
   (** Retrieve from a prophetic lender *)
-  Lemma plend_tok_retrieve {sm X α xπ Φx} :
-    [†α] -∗ plend_tok (X:=X) α xπ Φx -∗ modw M (pborrow_wsat M sm)
-      (plend_body sm xπ Φx).
+  Lemma plend_tok_retrieve {δ X α xπ Φx} :
+    [†α] -∗ plend_tok (X:=X) α xπ Φx -∗ modw M (borrow_wsat M ⟦⟧(δ))
+      (xplend δ xπ Φx).
   Proof. exact: lend_tok_retrieve. Qed.
 
   (** Open a prophetic borrower *)
-  Lemma pbor_tok_open {sm X α q x ξ Φx} :
-    q.[α] -∗ pbor_tok (X:=X) α x ξ Φx -∗ modw M (pborrow_wsat M sm)
-      (pobor_tok α q ξ Φx ∗ sm (Φx x)).
+  Lemma pbor_tok_open {δ X α q x ξ Φx} :
+    q.[α] -∗ pbor_tok (X:=X) α x ξ Φx -∗ modw M (borrow_wsat M ⟦⟧(δ))
+      (pobor_tok α q ξ Φx ∗ ⟦ Φx x ⟧(δ)).
   Proof.
     rewrite pbor_tok_unseal pobor_tok_unseal. iIntros "α [†|[%[vo b]]]".
     { iDestruct (lft_live_dead with "α †") as %[]. }
-    iMod (bor_tok_open (M:=M) (sm:=pbsem _) with "α b") as "[o[%[pc Φx]]]".
+    iMod (bor_tok_open (M:=M) with "α b") as "/=[o[%[>pc Φx]]]".
     iModIntro. iDestruct (vo_pc_agree with "vo pc") as %<-. iFrame "Φx".
     iExists _. iFrame "o". iExists _. iFrame.
   Qed.
@@ -440,9 +236,9 @@ Section pborrow.
       r:∗[of_plist_prvar ηl] ∗
       ([∗ plist] '(_, _, ξ, _, f)' ∈ αqξΦxfl,
         ⟨π, π (Aprvar _ ξ) = f (app_plist_prvar π ηl)⟩) ∗
-      ([∗ list] '(α, q, Pb)' ∈
-        of_plist (λ _ '(γ, α, q, ξ, Φx, _)', (α, q, xpbor _ γ ξ Φx)') γαqξΦxfl,
-        β ⊑□ α ∗ obor_tok α q Pb) ∗
+      ([∗ list] '(α, q, Px)' ∈ of_plist
+        (λ _ '(γ, α, q, ξ, Φx, _)', (α, q, cif_xpbor γ ξ Φx)') γαqξΦxfl,
+        β ⊑□ α ∗ obor_tok α q Px) ∗
       ∀ yl', ⟨π, app_plist_prvar π ηl = yl'⟩ -∗
         [∗ plist] '(γ, _, _, ξ, _, f)' ∈ γαqξΦxfl, proph_ctrl γ (f yl') ξ.
   Proof.
@@ -457,46 +253,47 @@ Section pborrow.
     iIntros (yl') "#obs". iDestruct ("→pcl" with "obs") as "$". iApply "→pc".
     by iApply (proph_obs_impl with "obs")=> ? ->.
   Qed.
-  Local Lemma pbor_list_sem_to_obs_sem {sm Yl γl' ηl} {yΨxl : plist _ Yl} :
-    ([∗ list] Qb ∈ pbor_list (plist_zip γl' (plist_zip ηl yΨxl)), pbsem sm Qb)
-      ==∗ ∃ yl', ⟨π, app_plist_prvar π ηl = yl'⟩ ∗
-      [∗ plist] '(y', _, Ψx)' ∈ plist_zip yl' yΨxl, sm (Ψx y').
+  Local Lemma cif_xpbors_sem_to_obs_sem {δ Yl γl' ηl} {yΨxl : plist _ Yl} :
+    ([∗ list] Qx ∈ cif_xpbors (plist_zip γl' (plist_zip ηl yΨxl)), ⟦ Qx ⟧(δ))
+      ==∗◇ ∃ yl', ⟨π, app_plist_prvar π ηl = yl'⟩ ∗
+      [∗ plist] '(y', _, Ψx)' ∈ plist_zip yl' yΨxl, ⟦ Ψx y' ⟧(δ).
   Proof.
     elim: Yl γl' ηl yΨxl=>/=.
     { iIntros (_ [] _ _) "!>". iExists (). iSplit; [|done].
       by iApply proph_obs_true. }
     move=> Y Yl IH [γ' γl'] [η ηl] [[y Ψx] yΨxl].
-    iIntros "[[%y'[pc Ψx]] pborl]". iMod (IH with "pborl") as (yl') "[obs Ψxl]".
+    iIntros "[[%y'[>pc Ψx]] pborl]".
+    iMod (IH with "pborl") as (yl') "[obs Ψxl]".
     iExists (y', yl')'. iFrame "Ψx Ψxl". iMod (pc_resolve with "pc") as "obs'".
     iModIntro. by iApply (proph_obs_impl2 with "obs obs'")=>/= ? <- <-.
   Qed.
   (** Merge and subdivide prophetic borrowers *)
-  Lemma pobor_tok_merge_subdiv {sm} Xl Yl
+  Lemma pobor_tok_merge_subdiv {δ} Xl Yl
     (αqξΦxfl : plist (λ X, _ *' _ *' _ *' _ *' (_ → X)) Xl) (yΨxl : plist _ Yl)
     Rxl β :
     ([∗ plist] '(α, q, ξ, Φx, _)' ∈ αqξΦxfl, β ⊑□ α ∗ pobor_tok α q ξ Φx) -∗
-    ([∗ plist] '(y, Ψx)' ∈ yΨxl, sm (Ψx y)) -∗ ([∗ list] Rx ∈ Rxl, sm Rx) -∗
+    ([∗ plist] '(y, Ψx)' ∈ yΨxl, ⟦ Ψx y ⟧(δ)) -∗
+    ([∗ list] Rx ∈ Rxl, ⟦ Rx ⟧(δ)) -∗
     (∀ yl', [†β] -∗
-      ([∗ plist] '(y', _, Ψx)' ∈ plist_zip yl' yΨxl, sm (Ψx y')) -∗
-      ([∗ list] Rx ∈ Rxl, sm Rx) -∗ M
-        ([∗ plist] '(_, _, _, Φx, f)' ∈ αqξΦxfl, sm (Φx (f yl'))))
-      =[pborrow_wsat M sm]=∗ ∃ ηl,
+      ([∗ plist] '(y', _, Ψx)' ∈ plist_zip yl' yΨxl, ⟦ Ψx y' ⟧(δ)) -∗
+      ([∗ list] Rx ∈ Rxl, ⟦ Rx ⟧(δ)) -∗ M
+        ([∗ plist] '(_, _, _, Φx, f)' ∈ αqξΦxfl, ⟦ Φx (f yl') ⟧(δ)))
+      =[borrow_wsat M ⟦⟧(δ)]=∗◇ ∃ ηl,
       ([∗ plist] '(α, q, _)' ∈ αqξΦxfl, q.[α]) ∗
       ([∗ plist] '(_, _, ξ, _, f)' ∈ αqξΦxfl,
         ⟨π, π (Aprvar _ ξ) = f (app_plist_prvar π ηl)⟩) ∗
       ([∗ plist] '(η, y, Ψx)' ∈ plist_zip ηl yΨxl, pbor_tok β y η Ψx) ∗
-      [∗ list] Rx ∈ Rxl, nbor_tok β Rx.
+      [∗ list] Rx ∈ Rxl, bor_tok β Rx.
   Proof.
     iIntros "ol Ψxl Rxl →Φxl".
     iMod (proph_alloc_list (plist_map (λ _, fst') yΨxl)) as (ηl) "ηl".
-    iExists ηl.
-    iMod (pobor_preresolve with "ηl ol") as (γl) "[ηl[$[ol →pcl]]]".
+    iExists ηl. iMod (pobor_preresolve with "ηl ol") as (γl) "[ηl[$[ol →pcl]]]".
     iMod (vo_pbor_alloc_list with "ηl Ψxl") as (γl') "[vol pborl]".
-    iMod (obor_tok_merge_subdiv (M:=M) (sm:=pbsem _) _
-      (_ ++ (xjustf <$> Rxl)) with "ol [pborl Rxl] [→Φxl →pcl]")
-      as "[αl bl]"; rewrite big_sepL_app !big_sepL_fmap. { by iFrame. }
+    iMod (obor_tok_merge_subdiv (M:=M) _ (_ ++ _)
+      with "ol [pborl Rxl] [→Φxl →pcl]") as "[αl bl]"; rewrite big_sepL_app.
+    { by iStopProof. }
     { iIntros "† [pborl Rxl]".
-      iMod (pbor_list_sem_to_obs_sem with "pborl") as (yl') "[obs Ψxl]".
+      iMod (cif_xpbors_sem_to_obs_sem with "pborl") as (yl') "[obs Ψxl]".
       iMod ("→Φxl" with "† Ψxl Rxl") as "Φxl". iModIntro.
       iDestruct ("→pcl" with "obs") as "pcl".
       rewrite big_sepL_of_plist
@@ -513,17 +310,17 @@ Section pborrow.
     rewrite pbor_tok_unseal. iRight. iExists _. iFrame.
   Qed.
   (** Subdivide a prophetic borrower *)
-  Lemma pobor_tok_subdiv {sm X α q ξ Φx} Yl (f : _ → X) (yΨxl : plist _ Yl) Rxl
+  Lemma pobor_tok_subdiv {δ X α q ξ Φx} Yl (f : _ → X) (yΨxl : plist _ Yl) Rxl
     β :
-    β ⊑□ α -∗ pobor_tok α q ξ Φx -∗ ([∗ plist] '(y, Ψx)' ∈ yΨxl, sm (Ψx y)) -∗
-    ([∗ list] Rx ∈ Rxl, sm Rx) -∗
+    β ⊑□ α -∗ pobor_tok α q ξ Φx -∗ ([∗ plist] '(y, Ψx)' ∈ yΨxl, ⟦ Ψx y ⟧(δ)) -∗
+    ([∗ list] Rx ∈ Rxl, ⟦ Rx ⟧(δ)) -∗
     (∀ yl', [†β] -∗
-      ([∗ plist] '(y', _, Ψx)' ∈ plist_zip yl' yΨxl, sm (Ψx y')) -∗
-      ([∗ list] Rx ∈ Rxl, sm Rx) -∗ M (sm (Φx (f yl'))))
-      =[pborrow_wsat M sm]=∗ ∃ ηl,
+      ([∗ plist] '(y', _, Ψx)' ∈ plist_zip yl' yΨxl, ⟦ Ψx y' ⟧(δ)) -∗
+      ([∗ list] Rx ∈ Rxl, ⟦ Rx ⟧(δ)) -∗ M ⟦ Φx (f yl') ⟧(δ))
+      =[borrow_wsat M ⟦⟧(δ)]=∗◇ ∃ ηl,
       q.[α] ∗ ⟨π, π (Aprvar _ ξ) = f (app_plist_prvar π ηl)⟩ ∗
       ([∗ plist] '(η, y, Ψx)' ∈ plist_zip ηl yΨxl, pbor_tok β y η Ψx) ∗
-      [∗ list] Rx ∈ Rxl, nbor_tok β Rx.
+      [∗ list] Rx ∈ Rxl, bor_tok β Rx.
   Proof.
     iIntros "⊑ o Ψxl Rxl →Φx".
     iMod (pobor_tok_merge_subdiv [_] _ ((_,_,_,_,_)',())'
@@ -533,33 +330,33 @@ Section pborrow.
   Qed.
 
   (** Resolve the prophecy of a prophetic borrower *)
-  Lemma pobor_tok_resolve {sm X α q ξ Φx} x :
-    pobor_tok (X:=X) α q ξ Φx -∗ sm (Φx x) =[pborrow_wsat M sm]=∗
-      q.[α] ∗ ⟨π, π ξ = x⟩ ∗ nbor_tok α (Φx x).
+  Lemma pobor_tok_resolve {δ X α q ξ Φx} x :
+    pobor_tok (X:=X) α q ξ Φx -∗ ⟦ Φx x ⟧(δ) =[borrow_wsat M ⟦⟧(δ)]=∗◇
+      q.[α] ∗ ⟨π, π ξ = x⟩ ∗ bor_tok α (Φx x).
   Proof.
     iIntros "o Φx".
     iMod (pobor_tok_subdiv [] (λ _, x) () [Φx x] with "[] o [//] [Φx] []")
       as (?) "[$[$[_[$ _]]]]"=>/=;
       by [iApply lft_sincl_refl|iFrame|iIntros "% _ _ [$ _]"|].
   Qed.
-  Lemma pbor_tok_resolve {sm X α q x ξ Φx} :
-    q.[α] -∗ pbor_tok (X:=X) α x ξ Φx -∗ modw M (pborrow_wsat M sm)
-      (q.[α] ∗ ⟨π, π ξ = x⟩ ∗ nbor_tok α (Φx x)).
+  Lemma pbor_tok_resolve {δ X α q x ξ Φx} :
+    q.[α] -∗ pbor_tok (X:=X) α x ξ Φx -∗ modw M (borrow_wsat M ⟦⟧(δ))
+      (q.[α] ∗ ⟨π, π ξ = x⟩ ∗ bor_tok α (Φx x)).
   Proof.
     iIntros "α b". iMod (pbor_tok_open with "α b") as "[o Φx]".
     by iMod (pobor_tok_resolve with "o Φx").
   Qed.
 
   (** Subdivide a prophetic borrower without changing the prophecy *)
-  Lemma pobor_tok_nsubdiv {sm X α q ξ Φx} Ψx x β :
-    β ⊑□ α -∗ pobor_tok (X:=X) α q ξ Φx -∗ sm (Ψx x) -∗
-    (∀ x', [†β] -∗ sm (Ψx x') -∗ M (sm (Φx x'))) =[pborrow_wsat M sm]=∗
+  Lemma pobor_tok_nsubdiv {δ X α q ξ Φx} Ψx x β :
+    β ⊑□ α -∗ pobor_tok (X:=X) α q ξ Φx -∗ ⟦ Ψx x ⟧(δ) -∗
+    (∀ x', [†β] -∗ ⟦ Ψx x' ⟧(δ) -∗ M ⟦ Φx x' ⟧(δ)) =[borrow_wsat M ⟦⟧(δ)]=∗
       q.[α] ∗ pbor_tok β x ξ Ψx.
   Proof.
     rewrite pobor_tok_unseal pbor_tok_unseal.
     iIntros "⊑ [%[[%[vo pc]] o]] Ψx →Φx".
     iMod (vo_pc_update with "vo pc") as "[vo pc]".
-    iMod (obor_tok_subdiv (M:=M) (sm:=pbsem _) [xpbor _ _ _ Ψx]
+    iMod (obor_tok_subdiv (FML:=cifOF _) (M:=M) [cif_xpbor _ _ Ψx]
       with "⊑ o [pc Ψx] [→Φx]") as "[$[_[? _]]]"=>/=.
     { iSplit; [|done]. iExists _. iFrame. }
     { iIntros "† [[%[pc Ψx]]_]". iMod ("→Φx" with "† Ψx") as "Φx". iModIntro.
@@ -567,8 +364,8 @@ Section pborrow.
     iModIntro. iRight. iExists _. iFrame.
   Qed.
   (** Simply close a prophetic borrower *)
-  Lemma pobor_tok_close {sm X α q ξ Φx} x :
-    pobor_tok (X:=X) α q ξ Φx -∗ sm (Φx x) =[pborrow_wsat M sm]=∗
+  Lemma pobor_tok_close {δ X α q ξ Φx} x :
+    pobor_tok (X:=X) α q ξ Φx -∗ ⟦ Φx x ⟧(δ) =[borrow_wsat M ⟦⟧(δ)]=∗
       q.[α] ∗ pbor_tok α x ξ Φx.
   Proof.
     iIntros "o Φx". iApply (pobor_tok_nsubdiv Φx with "[] o Φx"); [|by iIntros].
@@ -576,28 +373,28 @@ Section pborrow.
   Qed.
 
   (** Reborrow a nested prophetic borrower *)
-  Lemma pobor_pobor_tok_reborrow {sm X Y α q ξ Φx β r η Ψx} y f : β ⊑□ α -∗
-    pobor_tok (X:=X) β q ξ Φx -∗ pobor_tok (X:=Y) α r η Ψx -∗ sm (Ψx y) -∗
-    (∀ y', [†β] -∗ pbor_tok α y' η Ψx -∗ M (sm (Φx (f y')))) -∗
-      modw M (pborrow_wsat M sm) (∃ η' : prvar _,
+  Lemma pobor_pobor_tok_reborrow {δ X Y α q ξ Φx β r η Ψx} y f : β ⊑□ α -∗
+    pobor_tok (X:=X) β q ξ Φx -∗ pobor_tok (X:=Y) α r η Ψx -∗ ⟦ Ψx y ⟧(δ) -∗
+    (∀ y', [†β] -∗ pbor_tok α y' η Ψx -∗ M ⟦ Φx (f y') ⟧(δ)) -∗
+      modw M (borrow_wsat M ⟦⟧(δ)) (∃ η' : prvar _,
       q.[β] ∗ r.[α] ∗ ⟨π, π ξ = f (π η')⟩ ∗ pbor_tok β y η' Ψx).
   Proof.
     rewrite pobor_tok_unseal.
     iIntros "#⊑ [%γ[[%[vo pc]] o]] [%γ'[[%[vo' pc']] o']] Ψx →Φx".
     iMod (vo_pc_update with "vo pc") as "[vo pc]".
     iMod (vo_pc_update with "vo' pc'") as "[vo' pc']".
-    iMod (obor_tok_reborrow (M:=M) (sm:=pbsem _) β with "⊑ o' [pc' Ψx]")
-      as "($ & →b' & b)". { iExists _. iFrame. }
+    iMod (obor_tok_reborrow (M:=M) β with "⊑ o' [pc' Ψx]") as "($ & →b' & b)".
+    { iExists _. iFrame. }
     iMod vo_vo_alloc as (γx) "[vox vox']".
-    iMod (obor_tok_subdiv (M:=M) (sm:=pbsem _) [xpreborrow _ _ γ γ' γx ξ f]
+    iMod (obor_tok_subdiv (FML:=cifOF _) (M:=M)
+      [▷ ∃ y, proph_ctrl γ (f y) ξ ∗ val_obs γ' y ∗ val_obs γx y]%cif
       with "[] o [pc vo' vox'] [→Φx →b']") as "[[β β'][_[b' _]]]"=>/=.
     { iApply lft_sincl_refl. } { iSplit; [|done]. iExists _. iFrame. }
-    { iIntros "#† [[%y'[pc[vo' _]]]_]". iExists (f y'). iFrame "pc".
+    { iIntros "#† [>[%y'[pc[vo' _]]]_]". iExists (f y'). iFrame "pc".
       iApply ("→Φx" with "†"). rewrite pbor_tok_unseal. iRight. iExists _.
       iFrame "vo'". by iApply "→b'". }
-    iMod (bor_tok_open (M:=M) (sm:=pbsem _) with "β b") as "[o[%[pc' Ψx]]]".
-    iMod (bor_tok_open (M:=M) (sm:=pbsem _) with "β' b'")
-      as "[o'[%[pc[vo' vox']]]]".
+    iMod (bor_tok_open (M:=M) with "β b") as "/=[o [%[>pc' Ψx]]]".
+    iMod (bor_tok_open (M:=M) with "β' b'") as "/=[o' >[%[pc[vo' vox']]]]".
     iDestruct (vo_vo_agree with "vox vox'") as %<-.
     iDestruct (vo_pc_agree with "vo' pc'") as %<-.
     iMod (proph_alloc y) as (η') "η'". iExists η'.
@@ -605,12 +402,12 @@ Section pborrow.
       as "[[η' _][$ →pc]]".
     { apply proph_dep_constr, proph_dep_one. }
     iMod (vo_pc_alloc with "η'") as (γ'') "[vo'' pc'']".
-    iMod (obor_tok_merge_subdiv (M:=M) (sm:=pbsem _) [(_,_,_)';(_,_,_)']
-      [xpbor _ γ'' η' Ψx] with "[$o $o'] [pc'' Ψx] [→pc vo' pc' vox vox']")
+    iMod (obor_tok_merge_subdiv (FML:=cifOF _) (M:=M) [(_,_,_)';(_,_,_)']
+      [cif_xpbor γ'' η' Ψx] with "[$o $o'] [pc'' Ψx] [→pc vo' pc' vox vox']")
       as "[([$ _] & [$ _] & _) [b _]]"=>/=.
     { iSplit; [|iSplit=>//]; iApply lft_sincl_refl. }
     { iSplit; [|done]. iExists _. iFrame. }
-    { iIntros "_ [[%y'[pc'' Ψx]]_]". iMod (pc_resolve with "pc''") as "obs".
+    { iIntros "_ [[%y'[>pc'' Ψx]]_]". iMod (pc_resolve with "pc''") as "obs".
       iMod (vo_pc_update with "vo' pc'") as "[vo' pc']".
       iMod (vo_vo_update with "vox vox'") as "[vox _]". iModIntro.
       iSplitL "pc' Ψx"; [iExists _; by iFrame|]. iSplit; [|done]. iExists _.
@@ -618,10 +415,10 @@ Section pborrow.
       by iApply (proph_obs_impl with "obs")=> ? ->. }
     iModIntro. rewrite pbor_tok_unseal. iRight. iExists _. iFrame.
   Qed.
-  Lemma pobor_pbor_tok_reborrow {sm X Y α q ξ Φx β r y η Ψx} f : β ⊑□ α -∗
+  Lemma pobor_pbor_tok_reborrow {δ X Y α q ξ Φx β r y η Ψx} f : β ⊑□ α -∗
     pobor_tok (X:=X) β q ξ Φx -∗ r.[α] -∗ pbor_tok (X:=Y) α y η Ψx -∗
-    (∀ y', [†β] -∗ pbor_tok α y' η Ψx -∗ M (sm (Φx (f y')))) -∗
-      modw M (pborrow_wsat M sm) (∃ η' : prvar _,
+    (∀ y', [†β] -∗ pbor_tok α y' η Ψx -∗ M ⟦ Φx (f y') ⟧(δ)) -∗
+      modw M (borrow_wsat M ⟦⟧(δ)) (∃ η' : prvar _,
       q.[β] ∗ r.[α] ∗ ⟨π, π ξ = f (π η')⟩ ∗ pbor_tok β y η' Ψx).
   Proof.
     iIntros "⊑ Φx β b →Φx". iMod (pbor_tok_open with "β b") as "[o Ψx]".
@@ -629,11 +426,6 @@ Section pborrow.
   Qed.
 End pborrow.
 
-(** Allocate [pborrow_wsat] *)
-Lemma pborrow_wsat_alloc `{!pborrowGpreS TY FML Σ} :
-  ⊢ |==> ∃ _ : pborrowGS TY FML Σ, ∀ M sm, internal_ne sm -∗ pborrow_wsat M sm.
-Proof.
-  iMod proph_init as (?) "_". iMod borrow_wsat_alloc as (?) "big".
-  iModIntro. iExists (PborrowGS _ _ _ _ _ _). iIntros (??) "Ne". iApply "big".
-  by iApply pbsem_sem_ne.
-Qed.
+(** ** Notation *)
+Notation xplendd := (xplend der).
+Notation xplendd_var := (xplend_var der).
