nola/iris/pborrow_deriv.v
@@ -2,35 +2,35 @@
 
 From nola.util Require Import tagged.
 From nola.bi Require Export deriv.
-From nola.iris Require Export pborrow.
+From nola.iris Require Export pborrow borrow_deriv.
 From iris.proofmode Require Import proofmode.
 Import ProdNotation PlistNotation FunNPNotation iPropAppNotation ModwNotation
   LftNotation ProphNotation DsemNotation.
 
-Implicit Type (TY : synty) (FM : ofe).
+Implicit Type (TY : synty) (CON : cifcon) (Σ : gFunctors) (FM : ofe).
 
 (** ** [pborrow_judgty]: Judgment type for [pborrow] *)
-Variant pborrow_judg_id TY FM := .
-Definition pborrow_judgty TY (FM : ofe) : ofe := tagged (pborrow_judg_id TY FM)
-  ((** Basic conversion *) FM * FM +
+Variant pborrow_judg_id TY CON Σ := .
+Definition pborrow_judgty TY CON Σ : ofe := tagged (pborrow_judg_id TY CON Σ)
+  ((** Basic conversion *) cif CON Σ * cif CON Σ +
   (** Conversion judgment for [lend_body] *)
     @sigT (TY *' TY) (λ '(X, Y)',
       leibnizO (clair TY X *' clair TY Y) *
-      (X -d> FM) * (Y -d> FM)))%type.
+      (X -d> cif CON Σ) * (Y -d> cif CON Σ)))%type.
 
 (** ** [PborrowJudg]: Judgment structure for [pborrow] *)
-Notation PborrowJudg TY FM JUDG := (Ejudg (pborrow_judgty TY FM) JUDG).
+Notation PborrowJudg TY CON Σ JUDG := (Ejudg (pborrow_judgty TY CON Σ) JUDG).
 
 Section pborrow_deriv.
-  Context `{!pborrowGS TY FML Σ,
-    pborrow_judg : !PborrowJudg TY (FML $oi Σ) JUDG}.
-  Implicit Type (δ : JUDG -n> iProp Σ) (Px Qx : FML $oi Σ) (X Y : TY).
+  Context `{!borrowGS (cifOF CON) Σ, !prophGS TY Σ, !proph_agG TY Σ,
+    pborrow_judg : !PborrowJudg TY CON Σ JUDG}.
+  Implicit Type (δ : JUDG -n> iProp Σ) (Px Qx : cif CON Σ) (X Y : TY).
 
   (** Judgments *)
   Local Definition pborrow_jto Px Qx : JUDG :=
     pborrow_judg (Tagged (inl (Px, Qx))).
   Local Definition pborrow_jlto {X Y} (xπ : clair TY X) (yπ : clair TY Y)
-    (Φx : X -d> FML $oi Σ) (Ψx : Y -d> FML $oi Σ) : JUDG :=
+    (Φx : X -d> cif CON Σ) (Ψx : Y -d> cif CON Σ) : JUDG :=
     pborrow_judg (Tagged (inr (existT (X, Y)' ((xπ, yπ)', Φx, Ψx)))).
   #[export] Instance pborrow_jto_ne : NonExpansive2 pborrow_jto.
   Proof. solve_proper. Qed.
@@ -40,25 +40,6 @@ Section pborrow_deriv.
     unfold pborrow_jlto=> ???????. f_equiv. apply inr_ne. apply: existT_ne=>/=.
     split; [split|]; solve_proper.
   Qed.
-
-  (** [nbor]: Relaxed non-prophetic borrower *)
-  Local Definition nbor_def δ α Px : iProp Σ :=
-    ∃ Qx, □ δ (pborrow_jto Px Qx) ∗ □ δ (pborrow_jto Qx Px) ∗ nbor_tok α Qx.
-  Local Lemma nbor_aux : seal nbor_def. Proof. by eexists. Qed.
-  Definition nbor := nbor_aux.(unseal).
-  Local Lemma nbor_unseal : nbor = nbor_def. Proof. exact: seal_eq. Qed.
-  (** [nobor]: Relaxed non-prophetic open borrower *)
-  Local Definition nobor_def δ α q Px : iProp Σ :=
-    ∃ Qx, □ δ (pborrow_jto Px Qx) ∗ □ δ (pborrow_jto Qx Px) ∗ nobor_tok α q Qx.
-  Local Lemma nobor_aux : seal nobor_def. Proof. by eexists. Qed.
-  Definition nobor := nobor_aux.(unseal).
-  Local Lemma nobor_unseal : nobor = nobor_def. Proof. exact: seal_eq. Qed.
-  (** [nlend]: Relaxed non-prophetic lender *)
-  Local Definition nlend_def δ α Px : iProp Σ :=
-    ∃ Qx, □ δ (pborrow_jto Qx Px) ∗ nlend_tok α Qx.
-  Local Lemma nlend_aux : seal nlend_def. Proof. by eexists. Qed.
-  Definition nlend := nlend_aux.(unseal).
-  Local Lemma nlend_unseal : nlend = nlend_def. Proof. exact: seal_eq. Qed.
 
   (** [pbor]: Relaxed prophetic borrower *)
   Local Definition pbor_def {X} δ α x ξ (Φx : X -d> _) : iProp Σ :=
@@ -82,18 +63,6 @@ Section pborrow_deriv.
   Local Lemma plend_unseal : @plend = @plend_def. Proof. exact: seal_eq. Qed.
 
   (** Borrower and lender propositions are non-expansive *)
-  #[export] Instance nbor_ne {δ α} : NonExpansive (nbor δ α).
-  Proof. rewrite nbor_unseal. solve_proper. Qed.
-  #[export] Instance nbor_proper {δ α} : Proper ((≡) ==> (⊣⊢)) (nbor δ α).
-  Proof. apply ne_proper, _. Qed.
-  #[export] Instance nobor_ne {δ α q} : NonExpansive (nobor δ α q).
-  Proof. rewrite nobor_unseal. solve_proper. Qed.
-  #[export] Instance nobor_proper {δ α q} : Proper ((≡) ==> (⊣⊢)) (nobor δ α q).
-  Proof. apply ne_proper, _. Qed.
-  #[export] Instance nlend_ne {δ α} : NonExpansive (nlend δ α).
-  Proof. rewrite nlend_unseal. solve_proper. Qed.
-  #[export] Instance nlend_proper {δ α} : Proper ((≡) ==> (⊣⊢)) (nlend δ α).
-  Proof. apply ne_proper, _. Qed.
   #[export] Instance pbor_ne {δ X α x ξ} : NonExpansive (pbor (X:=X) δ α x ξ).
   Proof. rewrite pbor_unseal. solve_proper. Qed.
   #[export] Instance pbor_proper {δ X α x ξ} :
@@ -112,26 +81,19 @@ Section pborrow_deriv.
 End pborrow_deriv.
 
 (** Notation *)
-Notation nbord := (nbor der). Notation nobord := (nobor der).
-Notation nlendd := (nlend der).
 Notation pbord := (pbor der). Notation pobord := (pobor der).
 Notation plendd := (plend der).
-Notation plend_bodyi δ := (plend_body ⟦⟧(δ)).
-Notation plend_bodyid := (plend_bodyi der).
-Notation plend_body_vari δ := (plend_body_var ⟦⟧(δ)).
-Notation plend_body_varid := (plend_body_vari der).
 
 Section pborrow_deriv.
-  Context `{!pborrowGS TY FML Σ, !PborrowJudg TY (FML $oi Σ) JUDG,
-    !Jsem JUDG (iProp Σ), !Dsem JUDG (FML $oi Σ) (iProp Σ)}.
-  Implicit Type (δ : JUDG -n> iProp Σ) (Px Qx : FML $oi Σ).
+  Context `{!borrowGS (cifOF CON) Σ, !prophGS TY Σ, !proph_agG TY Σ,
+    !PborrowJudg TY CON Σ JUDG, !Jsem JUDG (iProp Σ), !SemCifcon JUDG CON Σ}.
+  Implicit Type (δ : JUDG -n> iProp Σ) (Px Qx : cif CON Σ).
 
   (** ** [pborrow_judg_sem]: Semantics of [pborrow_judgty] *)
-  Definition pborrow_judg_sem δ (J : pborrow_judgty TY (FML $oi Σ)) : iProp Σ :=
+  Definition pborrow_judg_sem δ (J : pborrow_judgty TY CON Σ) : iProp Σ :=
     match J.(untag) with
     | inl PQx => ⟦ PQx.1 ⟧(δ) ==∗ ⟦ PQx.2 ⟧(δ)
-    | inr (existT _ ((xπ, yπ)', Φx, Ψx)) =>
-        plend_body ⟦ ⟧(δ) xπ Φx ==∗ plend_body ⟦ ⟧(δ) yπ Ψx
+    | inr (existT _ ((xπ, yπ)', Φx, Ψx)) => xplend δ xπ Φx ==∗ xplend δ yπ Ψx
     end.
   (** [pborrow_judg_sem] is non-expansive *)
   #[export] Instance pborrow_judg_sem_ne {δ} :
@@ -142,19 +104,19 @@ Section pborrow_deriv.
   Qed.
   (** [Dsem] over [pborrow_judgty] *)
   #[export] Instance pborrow_jto_dsem
-    : Dsem JUDG (pborrow_judgty TY (FML $oi Σ)) (iProp Σ) :=
+    : Dsem JUDG (pborrow_judgty TY CON Σ) (iProp Σ) :=
     DSEM pborrow_judg_sem _.
 End pborrow_deriv.
 
 (** ** [PborrowJsem]: Judgment semantics for [pborrow] *)
-Notation PborrowJsem TY FML Σ JUDG :=
-  (Ejsem (pborrow_judgty TY (FML $oi Σ)) JUDG (iProp Σ)).
+Notation PborrowJsem TY CON Σ JUDG :=
+  (Ejsem (pborrow_judgty TY CON Σ) JUDG (iProp Σ)).
 
 Section pborrow_deriv.
-  Context `{!pborrowGS TY FML Σ, !PborrowJudg TY (FML $oi Σ) JUDG,
-    !Jsem JUDG (iProp Σ), !Dsem JUDG (FML $oi Σ) (iProp Σ),
-    !PborrowJsem TY FML Σ JUDG, !Deriv (JUDG:=JUDG) ih δ}.
-  Implicit Type (X Y Z : TY) (Px Qx Rx : FML $oi Σ) (δ : JUDG -n> iProp Σ).
+  Context `{!borrowGS (cifOF CON) Σ, !prophGS TY Σ, !proph_agG TY Σ,
+    !PborrowJudg TY CON Σ JUDG, !Jsem JUDG (iProp Σ), !SemCifcon JUDG CON Σ,
+    !PborrowJsem TY CON Σ JUDG, !Deriv (JUDG:=JUDG) ih δ}.
+  Implicit Type (X Y Z : TY) (Px Qx Rx : cif CON Σ) (δ : JUDG -n> iProp Σ).
 
   (** ** Conversion *)
 
@@ -192,7 +154,7 @@ Section pborrow_deriv.
   Qed.
   Local Lemma pborrow_jlto_trans {X Y Z xπ yπ zπ Φx Ψx Ω} :
     (∀ δ', ⌜Deriv ih δ'⌝ → ⌜ih δ'⌝ → ⌜dinto δ δ'⌝ →
-      plend_body ⟦ ⟧(δ') xπ Φx ==∗ plend_body ⟦ ⟧(δ') yπ Ψx) -∗
+      xplend δ' xπ Φx ==∗ xplend δ' yπ Ψx) -∗
     δ (pborrow_jlto (X:=Y) (Y:=Z) yπ zπ Ψx Ω) -∗
     δ (pborrow_jlto (X:=X) xπ zπ Φx Ω).
   Proof.
@@ -202,7 +164,7 @@ Section pborrow_deriv.
   Qed.
   Local Lemma pborrow_jlto_trans' {X Y Z xπ yπ zπ Φx Ψx Ω} :
     (∀ δ', ⌜Deriv ih δ'⌝ → ⌜ih δ'⌝ → ⌜dinto δ δ'⌝ →
-      plend_body ⟦ ⟧(δ') yπ Ψx ==∗ plend_body ⟦ ⟧(δ') zπ Ω) -∗
+      xplend δ' yπ Ψx ==∗ xplend δ' zπ Ω) -∗
     δ (pborrow_jlto (X:=X) (Y:=Y) xπ yπ Φx Ψx) -∗
     δ (pborrow_jlto (Y:=Z) xπ zπ Φx Ω).
   Proof.
@@ -212,40 +174,10 @@ Section pborrow_deriv.
   Qed.
   Local Lemma der_pborrow_jlto {X Y xπ yπ Φx Ψx} :
     der (pborrow_jlto (X:=X) (Y:=Y) xπ yπ Φx Ψx) ⊢
-      (plend_bodyid xπ Φx ==∗ plend_bodyid yπ Ψx).
+      (xplendd xπ Φx ==∗ xplendd yπ Ψx).
   Proof. by rewrite der_sound sem_ejudg. Qed.
 
   (** Convert the body of borrower and lender propositions *)
-  Lemma nbor_to {α Px Qx} :
-    □ (∀ δ', ⌜Deriv ih δ'⌝ → ⌜ih δ'⌝ → ⌜dinto δ δ'⌝ →
-      ⟦ Px ⟧(δ') ==∗ ⟦ Qx ⟧(δ')) -∗
-    □ (∀ δ', ⌜Deriv ih δ'⌝ → ⌜ih δ'⌝ → ⌜dinto δ δ'⌝ →
-      ⟦ Qx ⟧(δ') ==∗ ⟦ Px ⟧(δ')) -∗
-    nbor δ α Px -∗ nbor δ α Qx.
-  Proof.
-    rewrite nbor_unseal. iIntros "#PQ #QP (%Rx & #PR & #RP & $)".
-    iSplit; [iApply (pborrow_jto_trans with "QP PR")|
-      iApply (pborrow_jto_trans' with "PQ RP")].
-  Qed.
-  Lemma nobor_to {α q Px Qx} :
-    □ (∀ δ', ⌜Deriv ih δ'⌝ → ⌜ih δ'⌝ → ⌜dinto δ δ'⌝ →
-      ⟦ Px ⟧(δ') ==∗ ⟦ Qx ⟧(δ')) -∗
-    □ (∀ δ', ⌜Deriv ih δ'⌝ → ⌜ih δ'⌝ → ⌜dinto δ δ'⌝ →
-      ⟦ Qx ⟧(δ') ==∗ ⟦ Px ⟧(δ')) -∗
-    nobor δ α q Px -∗ nobor δ α q Qx.
-  Proof.
-    rewrite nobor_unseal. iIntros "#PQ #QP (%Rx & #PR & #RP & $)".
-    iSplit; [iApply (pborrow_jto_trans with "QP PR")|
-      iApply (pborrow_jto_trans' with "PQ RP")].
-  Qed.
-  Lemma nlend_to {α Px Qx} :
-    □ (∀ δ', ⌜Deriv ih δ'⌝ → ⌜ih δ'⌝ → ⌜dinto δ δ'⌝ →
-      ⟦ Px ⟧(δ') ==∗ ⟦ Qx ⟧(δ')) -∗
-    nlend δ α Px -∗ nlend δ α Qx.
-  Proof.
-    rewrite nlend_unseal. iIntros "#PQ (%Rx & #RP & $)".
-    iApply (pborrow_jto_trans' with "PQ RP").
-  Qed.
   Lemma pbor_to {X α x ξ Φx Ψx} :
     □ (∀ x' δ', ⌜Deriv ih δ'⌝ → ⌜ih δ'⌝ → ⌜dinto δ δ'⌝ →
       ⟦ Φx x' ⟧(δ') ==∗ ⟦ Ψx x' ⟧(δ')) -∗
@@ -270,7 +202,7 @@ Section pborrow_deriv.
   Qed.
   Lemma plend_to {X Y α xπ yπ Φx Ψx} :
     □ (∀ δ', ⌜Deriv ih δ'⌝ → ⌜ih δ'⌝ → ⌜dinto δ δ'⌝ →
-      plend_body ⟦ ⟧(δ') xπ Φx ==∗ plend_body ⟦ ⟧(δ') yπ Ψx) -∗
+      xplend δ' xπ Φx ==∗ xplend δ' yπ Ψx) -∗
     plend (X:=X) δ α xπ Φx -∗ plend (X:=Y) δ α yπ Ψx.
   Proof.
     rewrite plend_unseal. iIntros "#ΦΨ (%Z & %zπ & %Ω & #ΩΦ & $)".
@@ -278,22 +210,6 @@ Section pborrow_deriv.
   Qed.
 
   (** Modify the lifetime of borrower and lender propositions *)
-  Lemma nbor_lft {α β Px} : β ⊑□ α -∗ nbor δ α Px -∗ nbor δ β Px.
-  Proof.
-    rewrite nbor_unseal. iIntros "⊑ (% & #? & #? & b)".
-    iDestruct (nbor_tok_lft with "⊑ b") as "$". by iSplit.
-  Qed.
-  Lemma nobor_lft {α β q r Px} :
-    β ⊑□ α -∗ (q.[α] -∗ r.[β]) -∗ nobor δ α q Px -∗ nobor δ β r Px.
-  Proof.
-    rewrite nobor_unseal. iIntros "⊑ → (% & #? & #? & o)".
-    iDestruct (nobor_tok_lft with "⊑ → o") as "$". by iSplit.
-  Qed.
-  Lemma nlend_lft {α β Px} : α ⊑□ β -∗ nlend δ α Px -∗ nlend δ β Px.
-  Proof.
-    rewrite nlend_unseal. iIntros "⊑ (% & #? & l)".
-    by iDestruct (nlend_tok_lft with "⊑ l") as "$".
-  Qed.
   Lemma pbor_lft {X α β x ξ Φx} :
     β ⊑□ α -∗ pbor (X:=X) δ α x ξ Φx -∗ pbor δ β x ξ Φx.
   Proof.
@@ -314,16 +230,6 @@ Section pborrow_deriv.
   Qed.
 
   (** Turn from tokens *)
-  Lemma nbor_tok_nbor {α Px} : nbor_tok α Px ⊢ nbor δ α Px.
-  Proof.
-    rewrite nbor_unseal. iIntros "$". iSplit; iApply pborrow_jto_refl.
-  Qed.
-  Lemma nobor_tok_nobor {α q Px} : nobor_tok α q Px ⊢ nobor δ α q Px.
-  Proof.
-    rewrite nobor_unseal. iIntros "$". iSplit; iApply pborrow_jto_refl.
-  Qed.
-  Lemma nlend_tok_nlend {α Px} : nlend_tok α Px ⊢ nlend δ α Px.
-  Proof. rewrite nlend_unseal. iIntros "$". iApply pborrow_jto_refl. Qed.
   Lemma pbor_tok_pbor {X α x ξ Φx} :
     pbor_tok (X:=X) α x ξ Φx ⊢ pbor δ α x ξ Φx.
   Proof.
@@ -340,49 +246,28 @@ Section pborrow_deriv.
     plend_tok (X:=X) α xπ Φx ⊢ plend δ α xπ Φx.
   Proof. rewrite plend_unseal. iIntros "$". iApply pborrow_jlto_refl. Qed.
 
-  (** Fake a borrower *)
-  Lemma nbor_fake {α} Px : [†α] ⊢ nbor δ α Px.
-  Proof. by rewrite nbor_tok_fake nbor_tok_nbor. Qed.
-
-  Context `{!@ModUpd (iProp Σ) M, !ModBUpd M}.
+  Context `{!@ModUpd (iProp Σ) M, !ModBUpd M, !ModExcept0 M}.
 
   (** ** Rules that work under [Deriv ih δ] *)
-
-  (** Create borrowers and lenders *)
-  Lemma nbor_nlend_new_list α Pxl Qxl :
-    ([∗ list] Px ∈ Pxl, ⟦ Px ⟧(δ)) -∗
-    ([†α] -∗ ([∗ list] Px ∈ Pxl, ⟦ Px ⟧(δ)) -∗ M ([∗ list] Qx ∈ Qxl, ⟦ Qx ⟧(δ)))
-      =[pborrow_wsat M ⟦⟧(δ)]=∗
-      ([∗ list] Px ∈ Pxl, nbor δ α Px) ∗ [∗ list] Qx ∈ Qxl, nlend δ α Qx.
-  Proof.
-    setoid_rewrite <-nbor_tok_nbor. setoid_rewrite <-nlend_tok_nlend.
-    exact: nbor_nlend_tok_new_list.
-  Qed.
-  (** Simply create a borrower and a lender *)
-  Lemma nbor_nlend_new α Px :
-    ⟦ Px ⟧(δ) =[pborrow_wsat M ⟦⟧(δ)]=∗ nbor δ α Px ∗ nlend δ α Px.
-  Proof.
-    rewrite -nbor_tok_nbor -nlend_tok_nlend. exact: nbor_nlend_tok_new.
-  Qed.
 
   (** Create new prophetic borrowers and lenders *)
   Lemma pbor_plend_new_list α Xl (xΦxl : plist _ Xl) :
     ⊢ |==> ∃ ξl, ∀ Yl (yπΨxl : plist (λ Y, _ *' (Y → _)) Yl),
       let ξxΦxl := plist_zip ξl xΦxl in
       ([∗ plist] '(x, Φx)' ∈ xΦxl, ⟦ Φx x ⟧(δ)) -∗
-      ([†α] -∗ ([∗ plist] '(ξ, x, Φx)' ∈ ξxΦxl, plend_body_vari δ ξ Φx) -∗ M
-        ([∗ plist] '(yπ, Ψx)' ∈ yπΨxl, plend_bodyi δ yπ Ψx))
-        =[pborrow_wsat M ⟦⟧(δ)]=∗
+      ([†α] -∗ ([∗ plist] '(ξ, x, Φx)' ∈ ξxΦxl, xplend_var δ ξ Φx) -∗ M
+        ([∗ plist] '(yπ, Ψx)' ∈ yπΨxl, xplend δ yπ Ψx))
+        =[borrow_wsat M ⟦⟧(δ)]=∗◇
         ([∗ plist] '(ξ, x, Φx)' ∈ ξxΦxl, pbor δ α x ξ Φx) ∗
         ([∗ plist] '(yπ, Ψx)' ∈ yπΨxl, plend δ α yπ Ψx).
   Proof.
-    iMod (pbor_plend_tok_new_list (M:=M) (sm:=⟦⟧(_))) as (?) "big". iModIntro.
-    iExists _. iIntros (??). setoid_rewrite <-pbor_tok_pbor.
+    iMod (pbor_plend_tok_new_list (M:=M)) as (?) "big". iModIntro. iExists _.
+    iIntros (??). setoid_rewrite <-pbor_tok_pbor.
     setoid_rewrite <-plend_tok_plend. iApply "big".
   Qed.
   (** Simply create a prophetic borrower and a prophetic lender *)
   Lemma pbor_plend_new α X (x : X) Φx :
-    ⟦ Φx x ⟧(δ) =[pborrow_wsat M ⟦⟧(δ)]=∗ ∃ ξ,
+    ⟦ Φx x ⟧(δ) =[borrow_wsat M ⟦⟧(δ)]=∗◇ ∃ ξ,
       pbor δ α x ξ Φx ∗ plend δ α (λ π, π ξ) Φx.
   Proof.
     setoid_rewrite <-pbor_tok_pbor. setoid_rewrite <-plend_tok_plend.
@@ -391,124 +276,19 @@ Section pborrow_deriv.
 End pborrow_deriv.
 
 Section pborrow_deriv.
-  Context `{!pborrowGS TY FML Σ, !PborrowJudg TY (FML $oi Σ) JUDG,
-    !Jsem JUDG (iProp Σ), !Dsem JUDG (FML $oi Σ) (iProp Σ),
-    !PborrowJsem TY FML Σ JUDG, !@ModUpd (iProp Σ) M, !ModBUpd M}.
-  Implicit Type (X Y : TY) (Px Qx : FML $oi Σ).
-
-  (** ** On non-prophetic borrowing *)
-
-  (** Split a lender *)
-  Lemma nlendd_split {α Px} Qxl :
-    nlendd α Px -∗ (⟦ Px ⟧ -∗ M ([∗ list] Qx ∈ Qxl, ⟦ Qx ⟧))
-      =[pborrow_wsat M ⟦⟧]=∗ [∗ list] Qx ∈ Qxl, nlendd α Qx.
-  Proof.
-    rewrite {1}nlend_unseal. setoid_rewrite <-nlend_tok_nlend.
-    iIntros "(%Rx & #RP & l) →Ql".
-    iApply (nlend_tok_split (M:=M) with "l [RP →Ql]"). iIntros "Rx".
-    iMod (der_pborrow_jto with "RP Rx"). by iApply "→Ql".
-  Qed.
-
-  (** Retrive from [nlendd] *)
-  Lemma nlendd_retrieve {α Px} :
-    [†α] -∗ nlendd α Px -∗ modw M (pborrow_wsat M ⟦⟧) ⟦ Px ⟧.
-  Proof.
-    rewrite nlend_unseal. iIntros "† (%Qx & #QP & l)".
-    iMod (nlend_tok_retrieve (M:=M) with "† l") as "Qx".
-    iMod (der_pborrow_jto with "QP Qx") as "$". by iIntros.
-  Qed.
-
-  (** Open a borrower *)
-  Lemma nbord_open {α q Px} :
-    q.[α] -∗ nbord α Px -∗ modw M (pborrow_wsat M ⟦⟧) (nobord α q Px ∗ ⟦ Px ⟧).
-  Proof.
-    rewrite nbor_unseal nobor_unseal. iIntros "α (%Qx & $ & #QP & b)".
-    iMod (nbor_tok_open (M:=M) with "α b") as "[$ Qx]".
-    iMod (der_pborrow_jto with "QP Qx") as "$". by iIntros "$".
-  Qed.
-
-  (** Lemma for [nobord_merge_subdiv] *)
-  Local Lemma from_sincl_nobords {αqPxl β} :
-    ([∗ list] '(α, q, Px)' ∈ αqPxl, β ⊑□ α ∗ nobord α q Px) ⊢
-    ∃ αqRxl,
-      □ (([∗ list] '(_, _, Px)' ∈ αqPxl, ⟦ Px ⟧) ==∗
-        [∗ list] '(_, _, Rx)' ∈ αqRxl, ⟦ Rx ⟧) ∗
-      □ (([∗ list] '(α, q, Rx)' ∈ αqRxl, q.[α] ∗ ([†β] -∗ nbor_tok α Rx)) -∗
-        [∗ list] '(α, q, Px)' ∈ αqPxl, q.[α] ∗ ([†β] -∗ nbord α Px)) ∗
-      ([∗ list] '(α, q, Rx)' ∈ αqRxl, β ⊑□ α ∗ nobor_tok α q Rx).
-  Proof.
-    rewrite nobor_unseal /=. elim: αqPxl=>/=.
-    { iIntros. iExists []=>/=. do 2 (iSplit; [done|]). by iIntros. }
-    iIntros ([α[q Px]] αqPxl ->).
-    iIntros "[[⊑(%Rx & #PR & #RP & o)] (%αqRxl & #→Rxl & #→αbdl & ol)]".
-    iExists ((α, q, Rx)' :: αqRxl)=>/=. iFrame "⊑ o ol". iSplit.
-    - iIntros "!> [Px Pxl]". iMod ("→Rxl" with "Pxl") as "$".
-      iApply (der_pborrow_jto with "PR Px").
-    - iIntros "!> [[$ →b]αbl]". iDestruct ("→αbdl" with "αbl") as "$".
-      iIntros "†". rewrite nbor_unseal. iDestruct ("→b" with "†") as "$".
-      by iSplit.
-  Qed.
-  (** Merge and subdivide/reborrow borrowers *)
-  Lemma nobord_merge_subdiv αqPxl Qxl β :
-    ([∗ list] '(α, q, Px)' ∈ αqPxl, β ⊑□ α ∗ nobord α q Px) -∗
-    ([∗ list] Qx ∈ Qxl, ⟦ Qx ⟧) -∗
-    ([†β] -∗ ([∗ list] Qx ∈ Qxl, ⟦ Qx ⟧) -∗ M
-      ([∗ list] '(_, _, Px)' ∈ αqPxl, ⟦ Px ⟧)) =[pborrow_wsat M ⟦⟧]=∗
-      ([∗ list] '(α, q, Px)' ∈ αqPxl, q.[α] ∗ ([†β] -∗ nbord α Px)) ∗
-      ([∗ list] Qx ∈ Qxl, nbord β Qx).
-  Proof.
-    iIntros "big Qxl →Pxl". rewrite from_sincl_nobords /=.
-    iDestruct "big" as (αqRxl) "(#→Rxl & #→αbdl & ol)".
-    setoid_rewrite <-(nbor_tok_nbor (α:=β)).
-    iMod (nobor_tok_merge_subdiv (M:=M) with "ol Qxl [→Pxl]") as "[αbl $]".
-    - iIntros "† Qxl". iMod ("→Pxl" with "† Qxl") as "Pxl".
-      by iMod ("→Rxl" with "Pxl").
-    - iModIntro. by iApply "→αbdl".
-  Qed.
-  (** Subdivide/reborrow a borrower *)
-  Lemma nobord_subdiv {α q Px} Qxl β :
-    β ⊑□ α -∗ nobord α q Px -∗ ([∗ list] Qx ∈ Qxl, ⟦ Qx ⟧) -∗
-    ([†β] -∗ ([∗ list] Qx ∈ Qxl, ⟦ Qx ⟧) -∗ M ⟦ Px ⟧) =[pborrow_wsat M ⟦⟧]=∗
-      q.[α] ∗ ([†β] -∗ nbord α Px) ∗ ([∗ list] Qx ∈ Qxl, nbord β Qx).
-  Proof.
-    iIntros "⊑ o Qxl →Px".
-    iMod (nobord_merge_subdiv [(_,_,_)'] with "[⊑ o] Qxl [→Px]")
-      as "[[[$$]_]$]"=>/=; by [iFrame|rewrite bi.sep_emp|].
-  Qed.
-
-  (** Reborrow a borrower *)
-  Lemma nobord_reborrow {α q Px} β :
-    β ⊑□ α -∗ nobord α q Px -∗ ⟦ Px ⟧ =[pborrow_wsat M ⟦⟧]=∗
-      q.[α] ∗ ([†β] -∗ nbord α Px) ∗ nbord β Px.
-  Proof.
-    iIntros "⊑ o Px".
-    iMod (nobord_subdiv [Px] with "⊑ o [Px] []") as "($ & $ & $ & _)"=>/=;
-      by [iFrame|iIntros "_ [$ _]"|].
-  Qed.
-  Lemma nbord_reborrow {α q Px} β :
-    β ⊑□ α -∗ q.[α] -∗ nbord α Px -∗ modw M (pborrow_wsat M ⟦⟧)
-      (q.[α] ∗ ([†β] -∗ nbord α Px) ∗ nbord β Px).
-  Proof.
-    iIntros "⊑ α b". iMod (nbord_open with "α b") as "[o Px]".
-    by iMod (nobord_reborrow with "⊑ o Px").
-  Qed.
-  (** Simply close a borrower *)
-  Lemma nobord_close {α q Px} :
-    nobord α q Px -∗ ⟦ Px ⟧ =[pborrow_wsat M ⟦⟧]=∗ q.[α] ∗ nbord α Px.
-  Proof.
-    iIntros "o Px".
-    iMod (nobord_reborrow with "[] o Px") as "($ & _ & $)";
-      by [iApply lft_sincl_refl|].
-  Qed.
-
-  (** ** On prophetic borrowing *)
+  Context `{!borrowGS (cifOF CON) Σ, !prophGS TY Σ, !proph_agG TY Σ,
+    !PborrowJudg TY CON Σ JUDG, !BorrowJudg (cif CON Σ) JUDG,
+    !Jsem JUDG (iProp Σ), !SemCifcon JUDG CON Σ, !PborrowJsem TY CON Σ JUDG,
+    !BorrowJsem (cifOF CON) Σ JUDG,
+    !@ModUpd (iProp Σ) M, !ModBUpd M, !ModExcept0 M}.
+  Implicit Type (X Y : TY) (Px Qx : cif CON Σ).
 
   (** Split a prophetic lender *)
   Lemma plendd_split {X α xπ} {Φx : X → _} Yl
     (yπΨxl : plist (λ Y, _ *' (Y → _)) Yl) :
     plendd α xπ Φx -∗
-    (plend_bodyid xπ Φx -∗ M ([∗ plist] '(yπ, Ψx)' ∈ yπΨxl, plend_bodyid yπ Ψx))
-      =[pborrow_wsat M ⟦⟧]=∗ [∗ plist] '(yπ, Ψx)' ∈ yπΨxl, plendd α yπ Ψx.
+    (xplendd xπ Φx -∗ M ([∗ plist] '(yπ, Ψx)' ∈ yπΨxl, xplendd yπ Ψx))
+      =[borrow_wsat M ⟦⟧]=∗◇ [∗ plist] '(yπ, Ψx)' ∈ yπΨxl, plendd α yπ Ψx.
   Proof.
     rewrite {1}plend_unseal. iIntros "(%Z & %zπ & %Ω & ΩΦ & l) →Ψxl".
     setoid_rewrite <-plend_tok_plend.
@@ -518,7 +298,7 @@ Section pborrow_deriv.
 
   (** Retrieve from a prophetic lender *)
   Lemma plendd_retrieve {X α xπ} {Φx : X → _} :
-    [†α] -∗ plendd α xπ Φx -∗ modw M (pborrow_wsat M ⟦⟧) (plend_bodyid xπ Φx).
+    [†α] -∗ plendd α xπ Φx -∗ modw M (borrow_wsat M ⟦⟧) (xplendd xπ Φx).
   Proof.
     rewrite {1}plend_unseal. iIntros "† (%Y & %yπ & %Ψx & ΨΦ & l)".
     iMod (plend_tok_retrieve (M:=M) with "† l") as "lb".
@@ -527,7 +307,7 @@ Section pborrow_deriv.
 
   (** Open a prophetic borrower *)
   Lemma pbord_open {X α q x ξ} {Φx : X → _} :
-    q.[α] -∗ pbord α x ξ Φx -∗ modw M (pborrow_wsat M ⟦⟧)
+    q.[α] -∗ pbord α x ξ Φx -∗ modw M (borrow_wsat M ⟦⟧)
       (pobord α q ξ Φx ∗ ⟦ Φx x ⟧).
   Proof.
     rewrite pbor_unseal pobor_unseal. iIntros "α (% & $ & #ΨΦ & b)".
@@ -567,17 +347,17 @@ Section pborrow_deriv.
     (∀ yl', [†β] -∗ ([∗ plist] '(y', _, Ψx)' ∈ plist_zip yl' yΨxl, ⟦ Ψx y' ⟧) -∗
       ([∗ list] Rx ∈ Rxl, ⟦ Rx ⟧) -∗ M
         ([∗ plist] '(_, _, _, Φx, f)' ∈ αqξΦxfl, ⟦ Φx (f yl') ⟧))
-      =[pborrow_wsat M ⟦⟧]=∗ ∃ ηl,
+      =[borrow_wsat M ⟦⟧]=∗◇ ∃ ηl,
       ([∗ plist] '(α, q, _)' ∈ αqξΦxfl, q.[α]) ∗
       ([∗ plist] '(_, _, ξ, _, f)' ∈ αqξΦxfl,
         ⟨π, π (Aprvar _ ξ) = f (app_plist_prvar π ηl)⟩) ∗
       ([∗ plist] '(η, y, Ψx)' ∈ plist_zip ηl yΨxl, pbord β y η Ψx) ∗
-      [∗ list] Rx ∈ Rxl, nbord β Rx.
+      [∗ list] Rx ∈ Rxl, bord β Rx.
   Proof.
     rewrite from_sincl_pobords /=.
     iIntros "(% & %eq & %eq' & ol & →) Ψxl Rxl →Φxl". setoid_rewrite eq.
     setoid_rewrite eq'. setoid_rewrite <-pbor_tok_pbor.
-    setoid_rewrite <-nbor_tok_nbor.
+    setoid_rewrite <-bor_tok_bor.
     iApply (pobor_tok_merge_subdiv (M:=M) with "ol Ψxl Rxl").
     iIntros "% † Ψxl Rxl". iMod ("→Φxl" with "† Ψxl Rxl") as "Φxl".
     by iMod ("→" with "Φxl").
@@ -587,11 +367,11 @@ Section pborrow_deriv.
     β ⊑□ α -∗ pobord α q ξ Φx -∗
     ([∗ plist] '(y, Ψx)' ∈ yΨxl, ⟦ Ψx y ⟧) -∗ ([∗ list] Rx ∈ Rxl, ⟦ Rx ⟧) -∗
     (∀ yl', [†β] -∗ ([∗ plist] '(y', _, Ψx)' ∈ plist_zip yl' yΨxl, ⟦ Ψx y' ⟧) -∗
-      ([∗ list] Rx ∈ Rxl, ⟦ Rx ⟧) -∗ M ⟦ Φx (f yl') ⟧) =[pborrow_wsat M ⟦⟧]=∗
+      ([∗ list] Rx ∈ Rxl, ⟦ Rx ⟧) -∗ M ⟦ Φx (f yl') ⟧) =[borrow_wsat M ⟦⟧]=∗◇
       ∃ ηl,
       q.[α] ∗ ⟨π, π (Aprvar _ ξ) = f (app_plist_prvar π ηl)⟩ ∗
       ([∗ plist] '(η, y, Ψx)' ∈ plist_zip ηl yΨxl, pbord β y η Ψx) ∗
-      [∗ list] Rx ∈ Rxl, nbord β Rx.
+      [∗ list] Rx ∈ Rxl, bord β Rx.
   Proof.
     iIntros "⊑ o Ψxl Rxl →Φx".
     iMod (pobord_merge_subdiv [_] _ ((_,_,_,_,_)',())'
@@ -601,8 +381,8 @@ Section pborrow_deriv.
 
   (** Resolve the prophecy of a prophetic borrower *)
   Lemma pobord_resolve {X α q ξ Φx} (x : X) :
-    pobord α q ξ Φx -∗ ⟦ Φx x ⟧ =[pborrow_wsat M ⟦⟧]=∗
-      q.[α] ∗ ⟨π, π ξ = x⟩ ∗ nbord α (Φx x).
+    pobord α q ξ Φx -∗ ⟦ Φx x ⟧ =[borrow_wsat M ⟦⟧]=∗◇
+      q.[α] ∗ ⟨π, π ξ = x⟩ ∗ bord α (Φx x).
   Proof.
     iIntros "o Φx".
     iMod (pobord_subdiv [] (λ _, x) () [Φx x] with "[] o [//] [Φx] []")
@@ -610,8 +390,8 @@ Section pborrow_deriv.
       by [iApply lft_sincl_refl|iFrame|iIntros "% _ _ [$ _]"|].
   Qed.
   Lemma pbord_resolve {X α q x ξ} {Φx : X → _} :
-    q.[α] -∗ pbord α x ξ Φx -∗ modw M (pborrow_wsat M ⟦⟧)
-      (q.[α] ∗ ⟨π, π ξ = x⟩ ∗ nbord α (Φx x)).
+    q.[α] -∗ pbord α x ξ Φx -∗ modw M (borrow_wsat M ⟦⟧)
+      (q.[α] ∗ ⟨π, π ξ = x⟩ ∗ bord α (Φx x)).
   Proof.
     iIntros "α b". iMod (pbord_open with "α b") as "[o Φx]".
     iMod (pobord_resolve with "o Φx") as "$". by iIntros.
@@ -620,7 +400,7 @@ Section pborrow_deriv.
   (** Subdivide a prophetic borrower without changing the prophecy *)
   Lemma pobord_nsubdiv {X α q ξ Φx} Ψx (x : X) β :
     β ⊑□ α -∗ pobord α q ξ Φx -∗ ⟦ Ψx x ⟧ -∗
-    (∀ x', [†β] -∗ ⟦ Ψx x' ⟧ -∗ M ⟦ Φx x' ⟧) =[pborrow_wsat M ⟦⟧]=∗
+    (∀ x', [†β] -∗ ⟦ Ψx x' ⟧ -∗ M ⟦ Φx x' ⟧) =[borrow_wsat M ⟦⟧]=∗
       q.[α] ∗ pbord β x ξ Ψx.
   Proof.
     rewrite pobor_unseal. iIntros "⊑ (%Ω & #ΦΩ & _ & o) Ψx →Φx".
@@ -631,7 +411,7 @@ Section pborrow_deriv.
   Qed.
   (** Simply close a prophetic borrower *)
   Lemma pobord_close {X α q ξ Φx} (x : X) :
-    pobord α q ξ Φx -∗ ⟦ Φx x ⟧ =[pborrow_wsat M ⟦⟧]=∗ q.[α] ∗ pbord α x ξ Φx.
+    pobord α q ξ Φx -∗ ⟦ Φx x ⟧ =[borrow_wsat M ⟦⟧]=∗ q.[α] ∗ pbord α x ξ Φx.
   Proof.
     iIntros "o Φx". iApply (pobord_nsubdiv Φx with "[] o Φx"); [|by iIntros].
     iApply lft_sincl_refl.
@@ -641,7 +421,7 @@ Section pborrow_deriv.
   Lemma pobord_pobord_reborrow {X Y α q ξ Φx β r η Ψx} y (f : X → Y) :
     β ⊑□ α -∗ pobord β q ξ Φx -∗ pobord α r η Ψx -∗ ⟦ Ψx y ⟧ -∗
     (∀ y', [†β] -∗ pbord α y' η Ψx -∗ M ⟦ Φx (f y') ⟧) -∗
-      modw M (pborrow_wsat M ⟦⟧) (∃ η',
+      modw M (borrow_wsat M ⟦⟧) (∃ η',
       q.[β] ∗ r.[α] ∗ ⟨π, π ξ = f (π (Aprvar _ η'))⟩ ∗ pbord β y η' Ψx).
   Proof.
     rewrite pobor_unseal pbor_unseal.
@@ -656,7 +436,7 @@ Section pborrow_deriv.
   Lemma pobord_pbord_reborrow {X Y α q ξ Φx β r y η Ψx} (f : X → Y) :
     β ⊑□ α -∗ pobord β q ξ Φx -∗ r.[α] -∗ pbord α y η Ψx -∗
     (∀ y', [†β] -∗ pbord α y' η Ψx -∗ M ⟦ Φx (f y') ⟧) -∗
-      modw M (pborrow_wsat M ⟦⟧) (∃ η',
+      modw M (borrow_wsat M ⟦⟧) (∃ η',
         q.[β] ∗ r.[α] ∗ ⟨π, π ξ = f (π (Aprvar _ η'))⟩ ∗ pbord β y η' Ψx).
   Proof.
     iIntros "⊑ o r b →Φx". iMod (pbord_open with "r b") as "[o' Ψx]".
