nola/examples/borrow.v
@@ -8,32 +8,32 @@ Import ProdNotation FunPRNotation ModwNotation WpwNotation DsemNotation
 Section borrow.
   Context `{!lrustGS_gen hlc Σ, !SemCifcon JUDG CON Σ, !Jsem JUDG (iProp Σ),
     !inv'GS (cifOF CON) Σ, !InvCon CON, !InvSem JUDG CON Σ,
-    !pborrowGS nsynty (cifOF CON) Σ, !BorCon CON, !BorSem JUDG CON Σ}.
+    !borrowGS (cifOF CON) Σ, !BorCon CON, !BorSem JUDG CON Σ}.
   Implicit Type (Px Qx : cif CON Σ) (Φx Ψx : loc → cif CON Σ) (l : loc).
 
   (** Dereference a nested mutable reference *)
   Lemma bor_bor_deref {α β l Φx q} :
-    [[{ β ⊑□ α ∗ q.[β] ∗
-      nbor_tok β (∃ l', ▷ l ↦ #l' ∗ cif_bor α (Φx l'))%cif }]]
-      [pborrow_wsat bupd_0 ⟦⟧]
+    [[{ β ⊑□ α ∗ q.[β] ∗ bor_tok β (∃ l', ▷ l ↦ #l' ∗ cif_bor α (Φx l'))%cif }]]
+      [borrow_wsat bupd_0 ⟦⟧]
       !#l
-    [[{ l', RET #l'; q.[β] ∗ nbor_tok β (Φx l') }]].
+    [[{ l', RET #l'; q.[β] ∗ bor_tok β (Φx l') }]].
   Proof.
     iIntros (Ψ) "(#⊑ & [β β'] & b) →Ψ".
-    iMod (nbor_tok_open (M:=bupd_0) with "β b") as "/=[o [%l'[>↦ b']]]".
+    iMod (bor_tok_open (M:=bupd_0) with "β b") as "/=[o [%l'[>↦ b']]]".
     iApply twpw_fupdw_nonval; [done|]. wp_read.
     iMod (lft_sincl_live_acc with "⊑ β'") as (?) "[α →β']".
     rewrite sem_ecustom /=.
-    iMod (nbor_tok_reborrow (M:=bupd_0) with "⊑ α b'") as "(α & →b' & b')".
+    iMod (bor_tok_reborrow (M:=bupd_0) with "⊑ α b'") as "(α & →b' & b')".
     iDestruct ("→β'" with "α") as "β'".
-    iMod (nobor_tok_subdiv (M:=bupd_0) [] with "[] o [] [↦ →b']")
-      as "[β _]"=>/=. { iApply lft_sincl_refl. } { done. }
+    iMod (obor_tok_subdiv (M:=bupd_0) [] with "[] o [] [↦ →b']") as "[β _]"=>/=.
+    { iApply lft_sincl_refl. } { done. }
     { iIntros "† _ !>". iExists _. iFrame "↦". rewrite sem_ecustom /=.
       by iApply "→b'". }
     iModIntro. iApply "→Ψ". iFrame.
   Qed.
 
-  Context `{!PborCon nsynty CON, !PborSem nsynty JUDG CON Σ}.
+  Context `{!prophGS nsynty Σ, !proph_agG nsynty Σ, !PborCon nsynty CON,
+    !PborSem nsynty JUDG CON Σ}.
   Implicit Type X : nsynty.
 
   (** Dereference a nested prophetic mutable reference *)
@@ -41,7 +41,7 @@ Section borrow.
     [[{ β ⊑□ α ∗ q.[β] ∗
         pbor_tok β ((x, ξ)' : _ *'ₛ prvarₛ _) η
           (λ '(x', ξ')', ∃ l', ▷ l ↦ #l' ∗ cif_pbor α x' ξ' (Φxx l'))%cif }]]
-      [pborrow_wsat bupd_0 ⟦⟧]
+      [borrow_wsat bupd_0 ⟦⟧]
       !#l
     [[{ l', RET #l';
         q.[β] ∗ ∃ ξ' : prvar X,
@@ -61,14 +61,14 @@ Section borrow.
   (** Load from an immutable shared borrow *)
   Lemma imbor_load {l α q} {n : Z} :
     [[{ q.[α] ∗ inv_tok nroot (cif_bor α (▷ l ↦ #n)) }]]
-      [inv_wsat ⟦⟧ ∗ pborrow_wsat bupd_0 ⟦⟧]
+      [inv_wsat ⟦⟧ ∗ borrow_wsat bupd_0 ⟦⟧]
       !ˢᶜ#l
     [[{ RET #n; q.[α] }]].
   Proof.
     iIntros (Φ) "[α #i] →Φ". iMod (inv_tok_acc with "i") as "/=[b cl]"; [done|].
     rewrite sem_ecustom /=.
-    iMod (nbor_tok_open (M:=bupd_0) with "α b") as "/=[o >↦]". wp_read.
-    iMod (nobor_tok_close (M:=bupd_0) with "o [↦]") as "[α b]"=>/=; [done|].
+    iMod (bor_tok_open (M:=bupd_0) with "α b") as "/=[o >↦]". wp_read.
+    iMod (obor_tok_close (M:=bupd_0) with "o [↦]") as "[α b]"=>/=; [done|].
     iMod ("cl" with "b") as "_". iModIntro. by iApply "→Φ".
   Qed.
 End borrow.
